\documentclass[12pt]{article}
\usepackage[margin=1in]{geometry}
\usepackage{amsmath,amssymb}
\begin{document}

\section*{Problem 3}
If $x_1$ and $x_2$ are solutions of the quadratic equation $x^2 + x + 1 = 0$, and $y_1 = ax_1 + x_2$ and $y_2 = x_1 + ax_2$ (where $a \in \mathbb{R}$), then the solutions of the quadratic equation are:

\subsection*{Solution}
From the original equation $x^2 + x + 1 = 0$, by Vieta's formulas:
\begin{align}
x_1 + x_2 &= -1\\
x_1 \cdot x_2 &= 1
\end{align}

We have:
\begin{align}
y_1 &= ax_1 + x_2\\
y_2 &= x_1 + ax_2
\end{align}

Let's find the sum and product of $y_1$ and $y_2$:

Sum:
\begin{align}
y_1 + y_2 &= (ax_1 + x_2) + (x_1 + ax_2)\\
&= (a+1)x_1 + (a+1)x_2\\
&= (a+1)(x_1 + x_2)\\
&= (a+1)(-1) = -(a+1)
\end{align}

Product:
\begin{align}
y_1 \cdot y_2 &= (ax_1 + x_2)(x_1 + ax_2)\\
&= ax_1^2 + a^2x_1x_2 + x_1x_2 + ax_2^2\\
&= a(x_1^2 + x_2^2) + (a^2 + 1)x_1x_2
\end{align}

We need to find $x_1^2 + x_2^2$:
\[x_1^2 + x_2^2 = (x_1 + x_2)^2 - 2x_1x_2 = (-1)^2 - 2(1) = 1 - 2 = -1\]

Therefore:
\[y_1 \cdot y_2 = a(-1) + (a^2 + 1)(1) = -a + a^2 + 1 = a^2 - a + 1\]

The quadratic equation with roots $y_1$ and $y_2$ is:
\[y^2 - (y_1 + y_2)y + y_1y_2 = 0\]
\[y^2 - (-(a+1))y + (a^2 - a + 1) = 0\]
\[y^2 + (a+1)y + a^2 - a + 1 = 0\]

\subsection*{Answer}
$y^2 + (a+1)y + a^2 - a + 1 = 0$ (option \textbf{B}).

\end{document}