\documentclass[12pt]{article}
\usepackage[margin=1in]{geometry}
\usepackage{amsmath,amssymb}
\begin{document}

\section*{Problem 2}
Ako je $f(x) = x^2 + x + 1$, tada je $f(x + 2) - 2f(x + 1) + f(x)$ za svako $x$ jednako:

\subsection*{Solution}
Prvo ćemo naći izraze za $f(x+2)$, $f(x+1)$ i $f(x)$:

$f(x) = x^2 + x + 1$

$f(x+1) = (x+1)^2 + (x+1) + 1 = x^2 + 2x + 1 + x + 1 + 1 = x^2 + 3x + 3$

$f(x+2) = (x+2)^2 + (x+2) + 1 = x^2 + 4x + 4 + x + 2 + 1 = x^2 + 5x + 7$

Sada računamo:
$f(x + 2) - 2f(x + 1) + f(x)$
$= (x^2 + 5x + 7) - 2(x^2 + 3x + 3) + (x^2 + x + 1)$
$= x^2 + 5x + 7 - 2x^2 - 6x - 6 + x^2 + x + 1$
$= (x^2 - 2x^2 + x^2) + (5x - 6x + x) + (7 - 6 + 1)$
$= 0 + 0 + 2 = 2$

\subsection*{Answer}
$2$ (opcija \textbf{A}).

\end{document}