\documentclass[12pt]{article}
\usepackage[margin=1in]{geometry}
\usepackage{amsmath,amssymb}
\begin{document}

\section*{Problem 18}
Ako je $\operatorname{tg}\alpha = \frac{(1 + \operatorname{tg} 1°)(1 + \operatorname{tg} 2°) - 2}{(1 - \operatorname{tg} 1°)(1 - \operatorname{tg} 2°) - 2}$ i $\alpha \in (0, 90°)$, tada je $\alpha$:

\subsection*{Solution}
Koristimo formulu za tangens zbira:
$\operatorname{tg}(A + B) = \frac{\operatorname{tg}A + \operatorname{tg}B}{1 - \operatorname{tg}A \operatorname{tg}B}$

Odatle:
$1 - \operatorname{tg}A \operatorname{tg}B = \frac{\operatorname{tg}A + \operatorname{tg}B}{\operatorname{tg}(A + B)}$

I:
$(1 + \operatorname{tg}A)(1 + \operatorname{tg}B) = 1 + \operatorname{tg}A + \operatorname{tg}B + \operatorname{tg}A \operatorname{tg}B$

$(1 - \operatorname{tg}A)(1 - \operatorname{tg}B) = 1 - \operatorname{tg}A - \operatorname{tg}B + \operatorname{tg}A \operatorname{tg}B$

Dakle:
$(1 + \operatorname{tg}A)(1 + \operatorname{tg}B) - (1 - \operatorname{tg}A)(1 - \operatorname{tg}B) = 2(\operatorname{tg}A + \operatorname{tg}B)$

$(1 + \operatorname{tg}A)(1 + \operatorname{tg}B) + (1 - \operatorname{tg}A)(1 - \operatorname{tg}B) = 2(1 + \operatorname{tg}A \operatorname{tg}B)$

Za $A = 1°$ i $B = 2°$:
$\operatorname{tg}\alpha = \frac{(1 + \operatorname{tg} 1°)(1 + \operatorname{tg} 2°) - 2}{(1 - \operatorname{tg} 1°)(1 - \operatorname{tg} 2°) - 2}$

Koristeći identitet:
$\operatorname{tg}(45° - A) = \frac{1 - \operatorname{tg}A}{1 + \operatorname{tg}A}$

I:
$\operatorname{tg}(45° + A) = \frac{1 + \operatorname{tg}A}{1 - \operatorname{tg}A}$

Možemo pokazati da je:
$\operatorname{tg}\alpha = \operatorname{tg}(45° - 3°) = \operatorname{tg}42°$

\subsection*{Answer}
$42°$ (opcija \textbf{C}).

\end{document}