\documentclass[12pt]{article}
\usepackage[margin=1in]{geometry}
\usepackage{amsmath,amssymb}
\usepackage[utf8]{inputenc}

\begin{document}

\section*{Problem 1}
Vrednost izraza $\left(\frac{(-0,4)^3}{(-0,8)^3} - \frac{(-0,8)^3}{(-0,4)^3}\right) : \left(\frac{3}{4} - 3\right)$ jednaka je:

\subsection*{Solution}
We calculate the terms in the expression:
\[
\frac{(-0.4)^3}{(-0.8)^3} = \left(\frac{-0.4}{-0.8}\right)^3 = \left(\frac{1}{2}\right)^3 = \frac{1}{8}
\]
\[
\frac{(-0.8)^3}{(-0.4)^3} = \left(\frac{-0.8}{-0.4}\right)^3 = 2^3 = 8
\]
So the first bracket is:
\[
\frac{1}{8} - 8 = \frac{1 - 64}{8} = -\frac{63}{8}
\]
The second bracket is:
\[
\frac{3}{4} - 3 = \frac{3 - 12}{4} = -\frac{9}{4}
\]
Now divide the results:
\[
\left(-\frac{63}{8}\right) : \left(-\frac{9}{4}\right) = \frac{63}{8} \cdot \frac{4}{9} = \frac{63}{9} \cdot \frac{4}{8} = 7 \cdot \frac{1}{2} = \frac{7}{2}
\]

\subsection*{Answer}
(A) $\frac{7}{2}$

\end{document}
