\documentclass[12pt]{article}
\usepackage[margin=1in]{geometry}
\usepackage{amsmath,amssymb}
\begin{document}

\section*{Problem 9}
Find the sum of the first $2012$ terms of the arithmetic progression
\[
\frac{2011}{2012},\ \frac{2010}{2012},\ \frac{2009}{2012},\ \ldots
\]
Options: (A) $\frac{2013}{2}$ \quad (B) $\frac{2013}{4}$ \quad (C) $\frac{2011}{4}$ \quad (D) $\frac{2011}{2}$ \quad (E) none of the above.

\subsection*{Solution}
The first term is $a_1=\frac{2011}{2012}$ and the common difference is
\[
d=\frac{2010}{2012}-\frac{2011}{2012}=-\frac{1}{2012}.
\]
For $n=2012$, the sum is
\[
S_n=\frac{n}{2}\bigl(2a_1+(n-1)d\bigr)
=\frac{2012}{2}\left(2\cdot\frac{2011}{2012}+2011\cdot\left(-\frac{1}{2012}\right)\right).
\]
Inside the parentheses:
\[
2\cdot\frac{2011}{2012}-\frac{2011}{2012}=\frac{2011}{2012}.
\]
Hence
\[
S_{2012}=\frac{2012}{2}\cdot\frac{2011}{2012}=\frac{2011}{2}.
\]

\subsection*{Answer}
$\frac{2011}{2}$ (option \textbf{D}).

\end{document}

