\documentclass[12pt]{article}
\usepackage[margin=1in]{geometry}
\usepackage{amsmath,amssymb}
\begin{document}

\section*{Problem 1}
Compute the value of
\[
\left(\frac{(-0.4)^3}{(-0.8)^3}-\frac{(-0.8)^3}{(-0.4)^3}\right):\left(\frac34-3\right).
\]
Options: (A) $\frac72$ \quad (B) $\frac{63}{8}$ \quad (C) $\frac49$ \quad (D) $\frac59$ \quad (E) $\frac79$.

\subsection*{Solution}
Compute the two ratios:
\[
(-0.4)^3=-0.064,\quad (-0.8)^3=-0.512
\]
so
\[
\frac{(-0.4)^3}{(-0.8)^3}=\frac{-0.064}{-0.512}=\frac18,\qquad
\frac{(-0.8)^3}{(-0.4)^3}=\frac{-0.512}{-0.064}=8.
\]
Hence the numerator is
\[
\frac18-8=\frac18-\frac{64}{8}=-\frac{63}{8}.
\]
The divisor is
\[
\frac34-3=\frac34-\frac{12}{4}=-\frac94.
\]
Therefore
\[
\left(-\frac{63}{8}\right)\div\left(-\frac94\right)=\left(-\frac{63}{8}\right)\cdot\left(-\frac49\right)=\frac{252}{72}=\frac72.
\]

\subsection*{Answer}
$\frac72$ (option \textbf{A}).

\end{document}

