\documentclass[12pt]{article}
\usepackage[margin=1in]{geometry}
\usepackage{amsmath,amssymb}
\begin{document}

\section*{Problem 20}
Find the limit:
\[
\lim_{x \to 0} \frac{1 - \cos x \cos(2x) \cos(3x)}{1 - \cos x}
\]

\subsection*{Solution}
As $x \to 0$, both numerator and denominator approach 0, so we can use L'HÃ´pital's rule or Taylor expansions.

Using Taylor expansions around $x = 0$:
\[
\cos x = 1 - \frac{x^2}{2} + \frac{x^4}{24} + O(x^6)
\]
\[
\cos(2x) = 1 - \frac{(2x)^2}{2} + \frac{(2x)^4}{24} + O(x^6) = 1 - 2x^2 + \frac{2x^4}{3} + O(x^6)
\]
\[
\cos(3x) = 1 - \frac{(3x)^2}{2} + \frac{(3x)^4}{24} + O(x^6) = 1 - \frac{9x^2}{2} + \frac{27x^4}{8} + O(x^6)
\]

The denominator is:
\[
1 - \cos x = 1 - \left(1 - \frac{x^2}{2} + O(x^4)\right) = \frac{x^2}{2} + O(x^4)
\]

For the numerator, we need:
\[
\cos x \cos(2x) \cos(3x) = \left(1 - \frac{x^2}{2} + O(x^4)\right)\left(1 - 2x^2 + O(x^4)\right)\left(1 - \frac{9x^2}{2} + O(x^4)\right)
\]

Expanding to order $x^2$:
\[
\cos x \cos(2x) \cos(3x) = 1 - \left(\frac{1}{2} + 2 + \frac{9}{2}\right)x^2 + O(x^4) = 1 - 7x^2 + O(x^4)
\]

Therefore:
\[
1 - \cos x \cos(2x) \cos(3x) = 1 - (1 - 7x^2 + O(x^4)) = 7x^2 + O(x^4)
\]

The limit becomes:
\[
\lim_{x \to 0} \frac{7x^2 + O(x^4)}{\frac{x^2}{2} + O(x^4)} = \lim_{x \to 0} \frac{7x^2}{\frac{x^2}{2}} = \frac{7}{\frac{1}{2}} = 14
\]

\subsection*{Answer}
14 (option \textbf{B}).

\end{document}