\documentclass[12pt]{article}
\usepackage[margin=1in]{geometry}
\usepackage{amsmath,amssymb}
\begin{document}

\section*{Problem 13}
If the polynomial $x^{2016} + x^{2015} - x^{2014} + ax^{2013} - bx^2 + c$ (where $a, b, c \in \mathbb{R}$) is divisible by the polynomial $x^3 - x$, find the value of $4a^2 + 3b^2 + 8c^2$.

\subsection*{Solution}
If the polynomial $P(x) = x^{2016} + x^{2015} - x^{2014} + ax^{2013} - bx^2 + c$ is divisible by $x^3 - x = x(x-1)(x+1)$, then $P(0) = P(1) = P(-1) = 0$.

\textbf{From $P(0) = 0$:}
\[c = 0\]

\textbf{From $P(1) = 0$:}
\[1 + 1 - 1 + a - b + c = 0\]
\[1 + a - b + 0 = 0\]
\[a - b = -1 \quad \text{...(1)}\]

\textbf{From $P(-1) = 0$:}
\[(-1)^{2016} + (-1)^{2015} - (-1)^{2014} + a(-1)^{2013} - b(-1)^2 + c = 0\]
\[1 - 1 - 1 - a - b + 0 = 0\]
\[-1 - a - b = 0\]
\[a + b = -1 \quad \text{...(2)}\]

From (1) and (2):
\begin{align*}
a - b &= -1\\
a + b &= -1
\end{align*}

Adding: $2a = -2 \Rightarrow a = -1$

Subtracting: $2b = 0 \Rightarrow b = 0$

So $a = -1$, $b = 0$, $c = 0$.

Therefore:
\[4a^2 + 3b^2 + 8c^2 = 4(-1)^2 + 3(0)^2 + 8(0)^2 = 4 + 0 + 0 = 4\]

\subsection*{Answer}
$4$ (option \textbf{A}).

\end{document}
