\documentclass[12pt]{article}
\usepackage[margin=1in]{geometry}
\usepackage{amsmath,amssymb}
\begin{document}

\section*{Problem 1}
Ako je $a=2+\sqrt3$ i $b=2-\sqrt3$, odrediti vrednost izraza
\[
\Bigl((a+a^{-1})+(b+b^{-1})\Bigr)^{\frac12}.
\]

\subsection*{Solution}
Prvo primeÄ‡ujemo da je
\[
ab=(2+\sqrt3)(2-\sqrt3)=4-3=1 \quad\Rightarrow\quad b=\frac1a,\;\; a=\frac1b.
\]
Zato je
\[
a+a^{-1}=a+b,\qquad b+b^{-1}=b+a,
\]
pa je zbir
\[
(a+a^{-1})+(b+b^{-1})=2(a+b)=2\bigl((2+\sqrt3)+(2-\sqrt3)\bigr)=2\cdot 4=8.
\]
Dakle,
\[
\Bigl((a+a^{-1})+(b+b^{-1})\Bigr)^{\frac12}=\sqrt{8}=2\sqrt2.
\]

\subsection*{Answer}
$2\sqrt2$ (option \textbf{B}).

\end{document}

