\documentclass[12pt]{article}
\usepackage[margin=1in]{geometry}
\usepackage{amsmath,amssymb}
\begin{document}

\section*{Problem 12}
Zbir beskonačne geometrijske progresije
\[
\frac{\sqrt2+1}{\sqrt2-1}+\frac{1}{2-\sqrt2}+\frac12+\cdots
\]
jednak je:
\[
\text{(A)}~2+\sqrt2\quad
\text{(B)}~2-\sqrt2\quad
\text{(C)}~1\quad
\text{(D)}~4+3\sqrt2\quad
\text{(E)}~4-3\sqrt2.
\]

\subsection*{Solution}
Prvi član:
\[
a_1=\frac{\sqrt2+1}{\sqrt2-1}\cdot\frac{\sqrt2+1}{\sqrt2+1}
 =(\sqrt2+1)^2=3+2\sqrt2.
\]
Drugi član:
\[
a_2=\frac{1}{2-\sqrt2}\cdot\frac{2+\sqrt2}{2+\sqrt2}
=\frac{2+\sqrt2}{2}=1+\frac{\sqrt2}{2}.
\]
Odnos:
\[
r=\frac{a_2}{a_1}=\frac{\frac{2+\sqrt2}{2}}{3+2\sqrt2}
=\frac{2+\sqrt2}{2(3+2\sqrt2)}\cdot\frac{3-2\sqrt2}{3-2\sqrt2}
=\frac{2-\sqrt2}{2}.
\]
Provera: $a_3=a_2r=\dfrac{2+\sqrt2}{2}\cdot\dfrac{2-\sqrt2}{2}=\dfrac12$, što se slaže sa datim, pa je zaista geometrijska progresija.

Zbir beskonačne geometrijske progresije je
\[
S=\frac{a_1}{1-r}
=\frac{3+2\sqrt2}{1-\frac{2-\sqrt2}{2}}
=\frac{3+2\sqrt2}{\frac{\sqrt2}{2}}
=(3+2\sqrt2)\cdot\frac{2}{\sqrt2}=4+3\sqrt2.
\]

\subsection*{Answer}
$4+3\sqrt2$ (option \textbf{D}).

\end{document}

