\documentclass[12pt]{article}
\usepackage[margin=1in]{geometry}
\usepackage{amsmath,amssymb}
\usepackage[utf8]{inputenc}
\begin{document}

\section*{Problem 7}
Find the number of real solutions to the system:
\begin{align}
x^2 - 3xy + 5y^2 &= 1 \\
x^2 + xy + y^2 &= 1
\end{align}

\subsection*{Solution}
Let's solve this system by elimination.

From equation (2): $x^2 + xy + y^2 = 1$
From equation (1): $x^2 - 3xy + 5y^2 = 1$

Subtracting equation (2) from equation (1):
\[
(x^2 - 3xy + 5y^2) - (x^2 + xy + y^2) = 1 - 1
\]
\[
-4xy + 4y^2 = 0
\]
\[
4y(-x + y) = 0
\]

This gives us two cases:
1. $y = 0$
2. $y = x$

\textbf{Case 1:} $y = 0$

Substituting into equation (2):
\[
x^2 + x \cdot 0 + 0^2 = 1 \Rightarrow x^2 = 1 \Rightarrow x = \pm 1
\]

So we have solutions: $(1, 0)$ and $(-1, 0)$.

Let's verify in equation (1):
- For $(1, 0)$: $1^2 - 3(1)(0) + 5(0)^2 = 1$ ✓
- For $(-1, 0)$: $(-1)^2 - 3(-1)(0) + 5(0)^2 = 1$ ✓

\textbf{Case 2:} $y = x$

Substituting into equation (2):
\[
x^2 + x \cdot x + x^2 = 1 \Rightarrow 3x^2 = 1 \Rightarrow x^2 = \frac{1}{3} \Rightarrow x = \pm\frac{1}{\sqrt{3}}
\]

So we have solutions: $\left(\frac{1}{\sqrt{3}}, \frac{1}{\sqrt{3}}\right)$ and $\left(-\frac{1}{\sqrt{3}}, -\frac{1}{\sqrt{3}}\right)$.

Let's verify in equation (1):
- For $\left(\frac{1}{\sqrt{3}}, \frac{1}{\sqrt{3}}\right)$: 
  $\left(\frac{1}{\sqrt{3}}\right)^2 - 3\left(\frac{1}{\sqrt{3}}\right)\left(\frac{1}{\sqrt{3}}\right) + 5\left(\frac{1}{\sqrt{3}}\right)^2 = \frac{1}{3} - 3 \cdot \frac{1}{3} + 5 \cdot \frac{1}{3} = \frac{1 - 3 + 5}{3} = \frac{3}{3} = 1$ ✓

- For $\left(-\frac{1}{\sqrt{3}}, -\frac{1}{\sqrt{3}}\right)$: 
  $\left(-\frac{1}{\sqrt{3}}\right)^2 - 3\left(-\frac{1}{\sqrt{3}}\right)\left(-\frac{1}{\sqrt{3}}\right) + 5\left(-\frac{1}{\sqrt{3}}\right)^2 = \frac{1}{3} - 3 \cdot \frac{1}{3} + 5 \cdot \frac{1}{3} = 1$ ✓

Therefore, we have 4 real solutions in total.

\subsection*{Answer}
$4$ (option \textbf{A}).

\end{document}

