\documentclass[12pt]{article}
\usepackage[margin=1in]{geometry}
\usepackage{amsmath,amssymb}
\usepackage[utf8]{inputenc}
\usepackage[T1]{fontenc}

\begin{document}

\section*{Problem 9}
Ako je $f(x) = \left(\frac{x+1}{x-1}\right)^2$ ($x \ne \pm 1$) tada je $f\left(\frac{x+1}{x-1}\right) - f\left(\frac{x-1}{x+1}\right)$ jednako:
\[
(A)\; \left(\frac{x+1}{x-1}\right)^2 \quad (B)\; \left(\frac{x-1}{x+1}\right)^2 \quad (C)\; 0 \quad (D)\; \frac{x^2-1}{x^2+1} \quad (E)\; -\left(\frac{x-1}{x+1}\right)^2
\]

\subsection*{Solution}
Neka je $g(x) = \frac{x+1}{x-1}$. Tada je $f(x) = (g(x))^2$.
Prvi 훾lan izraza je $f(g(x)) = f\left(\frac{x+1}{x-1}\right)$.
Drugi 훾lan izraza je $f\left(\frac{1}{g(x)}\right) = f\left(\frac{x-1}{x+1}\right)$.
Izra훾unajmo $f(1/t)$ za $t = g(x)$:
\[
f(1/t) = \left(\frac{1/t + 1}{1/t - 1}\right)^2 = \left(\frac{\frac{1+t}{t}}{\frac{1-t}{t}}\right)^2 = \left(\frac{1+t}{1-t}\right)^2 = \left(\frac{t+1}{-(t-1)}\right)^2 = \left(\frac{t+1}{t-1}\right)^2 = f(t)
\]
Dakle, $f\left(\frac{x-1}{x+1}\right) = f\left(\frac{x+1}{x-1}\right)$.
Razlika ova dva 훾lana je:
\[
f\left(\frac{x+1}{x-1}\right) - f\left(\frac{x-1}{x+1}\right) = 0
\]

\subsection*{Answer}
$0$ (option \textbf{C}).

\end{document}
