\documentclass[12pt]{article}
\usepackage[margin=1in]{geometry}
\usepackage{amsmath,amssymb}
\begin{document}

\section*{Problem 13}
Sva realna rešenja iracionalne jednačine $\frac{1}{\sqrt{x}+\sqrt{x-2}} + \frac{1}{\sqrt{x+2}+\sqrt{x}} = \frac{1}{4}$ pripadaju skupu:
\begin{enumerate}
    \item[(A)] $[2, 6)$
    \item[(B)] $[6, 10)$
    \item[(C)] $[10, 14)$
    \item[(D)] $[14, 18)$
    \item[(E)] $[18, +\infty)$
    \item[(N)] Ne znam
\end{enumerate}

\subsection*{Solution}
Rationalize each term:
\[
\frac{1}{\sqrt{x}+\sqrt{x-2}} = \frac{\sqrt{x}-\sqrt{x-2}}{x-(x-2)} = \frac{\sqrt{x}-\sqrt{x-2}}{2}
\]
\[
\frac{1}{\sqrt{x+2}+\sqrt{x}} = \frac{\sqrt{x+2}-\sqrt{x}}{(x+2)-x} = \frac{\sqrt{x+2}-\sqrt{x}}{2}
\]
Summing them:
\[
\frac{\sqrt{x}-\sqrt{x-2} + \sqrt{x+2}-\sqrt{x}}{2} = \frac{\sqrt{x+2}-\sqrt{x-2}}{2}
\]
The equation becomes:
\[
\frac{\sqrt{x+2}-\sqrt{x-2}}{2} = \frac{1}{4} \implies \sqrt{x+2}-\sqrt{x-2} = \frac{1}{2}
\]
Square both sides:
\[
(x+2) - 2\sqrt{(x+2)(x-2)} + (x-2) = \frac{1}{4}
\]
\[
2x - 2\sqrt{x^2-4} = \frac{1}{4}
\]
\[
2\sqrt{x^2-4} = 2x - 0.25
\]
\[
\sqrt{x^2-4} = x - 0.125 = x - \frac{1}{8}
\]
Square again:
\[
x^2-4 = x^2 - \frac{x}{4} + \frac{1}{64}
\]
\[
-4 = -\frac{x}{4} + \frac{1}{64}
\]
\[
\frac{x}{4} = 4 + \frac{1}{64} = \frac{257}{64}
\]
\[
x = \frac{257}{16} = 16.0625
\]
The solution $16.0625$ lies in the interval $[14, 18)$.

\subsection*{Answer}
$[14, 18)$ (option \textbf{(D)}).

\end{document}