\documentclass[12pt]{article}
\usepackage[margin=1in]{geometry}
\usepackage{amsmath,amssymb}
\begin{document}

\section*{Problem 9}
Data je kvadratna funkcija $f(x) = x^2+bx+c$ ($b,c \in \mathbf{R}$) takva da je $f(f(1)) = f(f(2)) = 0$, pri ƒçemu je $f(1) \neq f(2)$. Vrednost $f(0)$ jednaka je:
\begin{enumerate}
    \item[(A)] $-6$
    \item[(B)] $-\frac{2}{3}$
    \item[(C)] $-\frac{3}{2}$
    \item[(D)] $\frac{1}{4}$
    \item[(E)] $-2$
    \item[(N)] Ne znam
\end{enumerate}

\subsection*{Solution}
Let $f(1) = u$ and $f(2) = v$. We are given $u \neq v$.
The condition $f(f(1)) = f(f(2)) = 0$ translates to $f(u) = 0$ and $f(v) = 0$.
Thus, $u$ and $v$ are the roots of the quadratic equation $f(x) = x^2+bx+c = 0$.
By Vieta's formulas:
\[
u+v = -b
\]
\[
uv = c
\]
Also, we can express $u$ and $v$ using the function definition:
\[
u = f(1) = 1+b+c
\]
\[
v = f(2) = 4+2b+c
\]
Substitute $c = uv$:
\[
u = 1+b+uv \quad (1)
\]
\[
v = 4+2b+uv \quad (2)
\]
Subtract (1) from (2):
\[
v-u = 3+b \implies b = v-u-3
\]
Substitute $b = -(u+v)$:
\[
v-u = 3 - (u+v) \implies v-u = 3-u-v \implies 2v = 3 \implies v = \frac{3}{2}
\]
Now find $b$:
\[
b = \frac{3}{2} - u - 3 = -u - \frac{3}{2}
\]
Since $b = -(u+v) = -(u+3/2)$, this is consistent.
Now use equation (1) with $b = -(u+3/2)$:
\[
u = 1 - (u+3/2) + u(3/2)
\]
\[
u = 1 - u - 3/2 + 3u/2 = -1/2 + u/2
\]
\[
u/2 = -1/2 \implies u = -1
\]
So the roots are $u = -1$ and $v = 3/2$.
Then $c = uv = (-1)(3/2) = -3/2$.
The value of $f(0)$ is $c$.
\[
f(0) = c = -3/2
\]

\subsection*{Answer}
$-\frac{3}{2}$ (option \textbf{(C)}).

\end{document}