\documentclass[12pt]{article}
\usepackage[margin=1in]{geometry}
\usepackage{amsmath,amssymb}
\begin{document}

\section*{Problem 1}
Vrednost izraza $2014^3 - 2013 \cdot 2014 \cdot 2015$ jednaka je:
\begin{enumerate}
    \item[(A)] $1$
    \item[(B)] $2013$
    \item[(C)] $2014$
    \item[(D)] $2015$
    \item[(E)] $-1$
    \item[(N)] Ne znam
\end{enumerate}

\subsection*{Solution}
Let $x = 2014$. The expression can be rewritten as:
\[
x^3 - (x-1) \cdot x \cdot (x+1)
\]
Simplifying the term $(x-1)x(x+1)$:
\[
(x-1)x(x+1) = x(x^2-1) = x^3 - x
\]
Now substitute back into the original expression:
\[
x^3 - (x^3 - x) = x^3 - x^3 + x = x
\]
Since $x = 2014$, the value is $2014$.

\subsection*{Answer}
$2014$ (option \textbf{(C)}).

\end{document}