\documentclass[12pt]{article}
\usepackage[utf8]{inputenc}
\usepackage[T2A]{fontenc}
\usepackage[serbian]{babel}
\usepackage{amsmath,amssymb}
\usepackage{geometry}
\geometry{a4paper, margin=2.5cm}

\begin{document}

\section*{Problem 12 - Solution}

\textbf{Problem:} If $f(x) - 2f\left(\frac{1}{x}\right) = x^2$, $x \neq 0$, find $f(2)$.

\textbf{Solution:}

We have the functional equation:
\[
f(x) - 2f\left(\frac{1}{x}\right) = x^2
\]

\textbf{Step 1:} Substitute $x = 2$:
\[
f(2) - 2f\left(\frac{1}{2}\right) = 4 \quad \text{...(1)}
\]

\textbf{Step 2:} Substitute $x = \frac{1}{2}$:
\[
f\left(\frac{1}{2}\right) - 2f(2) = \frac{1}{4} \quad \text{...(2)}
\]

\textbf{Step 3:} Solve the system

From equation (2):
\[
f\left(\frac{1}{2}\right) = \frac{1}{4} + 2f(2)
\]

Substitute into equation (1):
\[
f(2) - 2\left(\frac{1}{4} + 2f(2)\right) = 4
\]
\[
f(2) - \frac{1}{2} - 4f(2) = 4
\]
\[
-3f(2) = 4 + \frac{1}{2} = \frac{9}{2}
\]
\[
f(2) = -\frac{3}{2}
\]

\textbf{Answer: Ð”) $-\frac{3}{2}$}

\end{document}

