\documentclass[12pt]{article}
\usepackage[margin=1in]{geometry}
\usepackage{amsmath,amssymb}
\begin{document}

\section*{Problem 2}
Vrednost izraza $\left(\frac{i^{2011} + i^{2012}}{i^{2013} - i^{2014}}\right)^{2015}$, $(i^2 = -1)$, jednaka je:

(A) $-1$ \quad (B) $0$ \quad (C) $1$ \quad (D) $i$ \quad (E) $-i$ \quad (N) Ne znam

\subsection*{Solution}
First, let's find the pattern of powers of $i$:
\begin{align}
i^1 &= i\\
i^2 &= -1\\
i^3 &= i^2 \cdot i = -i\\
i^4 &= i^2 \cdot i^2 = (-1)(-1) = 1
\end{align}

The pattern repeats every 4 powers: $i^{4k+r} = i^r$ for $r \in \{0,1,2,3\}$.

Now let's calculate each power:
\begin{align}
2011 &= 4 \cdot 502 + 3 \Rightarrow i^{2011} = i^3 = -i\\
2012 &= 4 \cdot 503 + 0 \Rightarrow i^{2012} = i^0 = 1\\
2013 &= 4 \cdot 503 + 1 \Rightarrow i^{2013} = i^1 = i\\
2014 &= 4 \cdot 503 + 2 \Rightarrow i^{2014} = i^2 = -1
\end{align}

Substituting:
\begin{align}
\frac{i^{2011} + i^{2012}}{i^{2013} - i^{2014}} &= \frac{-i + 1}{i - (-1)} = \frac{1 - i}{i + 1}
\end{align}

To simplify this, multiply numerator and denominator by the conjugate of the denominator:
\begin{align}
\frac{1 - i}{i + 1} \cdot \frac{-i + 1}{-i + 1} &= \frac{(1 - i)(1 - i)}{(i + 1)(1 - i)}\\
&= \frac{(1 - i)^2}{1 - i^2}\\
&= \frac{1 - 2i + i^2}{1 - (-1)}\\
&= \frac{1 - 2i - 1}{2}\\
&= \frac{-2i}{2} = -i
\end{align}

Therefore:
$$\left(\frac{i^{2011} + i^{2012}}{i^{2013} - i^{2014}}\right)^{2015} = (-i)^{2015}$$

Since $2015 = 4 \cdot 503 + 3$, we have $(-i)^{2015} = (-i)^3 = (-1)^3 \cdot i^3 = (-1)(-i) = i$.

\subsection*{Answer}
(D) $i$

\end{document}