\documentclass[12pt]{article}
\usepackage[margin=1in]{geometry}
\usepackage{amsmath,amssymb}
\begin{document}

\section*{Problem 12}
Zbir beskonaƒçne geometrijske progresije $\frac{\sqrt{2} + 1}{\sqrt{2} - 1} + \frac{1}{2 - \sqrt{2}} + \frac{1}{2} + \cdots$ jednak je:

(A) $2 + \sqrt{2}$ \quad (B) $2 - \sqrt{2}$ \quad (C) $1$ \quad (D) $4 + 3\sqrt{2}$ \quad (E) $4 - 3\sqrt{2}$ \quad (N) Ne znam

\subsection*{Solution}
First, let's simplify the terms of the series.

For the first term, rationalize the denominator:
$$\frac{\sqrt{2} + 1}{\sqrt{2} - 1} = \frac{(\sqrt{2} + 1)(\sqrt{2} + 1)}{(\sqrt{2} - 1)(\sqrt{2} + 1)} = \frac{(\sqrt{2} + 1)^2}{2 - 1} = (\sqrt{2} + 1)^2 = 2 + 2\sqrt{2} + 1 = 3 + 2\sqrt{2}$$

For the second term:
$$\frac{1}{2 - \sqrt{2}} = \frac{2 + \sqrt{2}}{(2 - \sqrt{2})(2 + \sqrt{2})} = \frac{2 + \sqrt{2}}{4 - 2} = \frac{2 + \sqrt{2}}{2}$$

The third term is $\frac{1}{2}$.

Let's check if this is indeed a geometric progression by finding the common ratio.

From first to second term:
$$r = \frac{\frac{2 + \sqrt{2}}{2}}{3 + 2\sqrt{2}} = \frac{2 + \sqrt{2}}{2(3 + 2\sqrt{2})} = \frac{2 + \sqrt{2}}{6 + 4\sqrt{2}}$$

Let's rationalize:
$$r = \frac{(2 + \sqrt{2})(6 - 4\sqrt{2})}{(6 + 4\sqrt{2})(6 - 4\sqrt{2})} = \frac{12 - 8\sqrt{2} + 6\sqrt{2} - 8}{36 - 32} = \frac{4 - 2\sqrt{2}}{4} = \frac{2 - \sqrt{2}}{2}$$

From second to third term:
$$r = \frac{\frac{1}{2}}{\frac{2 + \sqrt{2}}{2}} = \frac{1}{2 + \sqrt{2}} = \frac{2 - \sqrt{2}}{(2 + \sqrt{2})(2 - \sqrt{2})} = \frac{2 - \sqrt{2}}{4 - 2} = \frac{2 - \sqrt{2}}{2}$$

So the common ratio is $r = \frac{2 - \sqrt{2}}{2}$.

Since $|r| = \frac{2 - \sqrt{2}}{2} < 1$ (because $2 - \sqrt{2} \approx 0.586 < 2$), the series converges.

The sum of an infinite geometric series is $S = \frac{a}{1 - r}$ where $a$ is the first term.

$$S = \frac{3 + 2\sqrt{2}}{1 - \frac{2 - \sqrt{2}}{2}} = \frac{3 + 2\sqrt{2}}{\frac{2 - (2 - \sqrt{2})}{2}} = \frac{3 + 2\sqrt{2}}{\frac{\sqrt{2}}{2}} = \frac{2(3 + 2\sqrt{2})}{\sqrt{2}}$$

Rationalizing:
$$S = \frac{2(3 + 2\sqrt{2})\sqrt{2}}{2} = (3 + 2\sqrt{2})\sqrt{2} = 3\sqrt{2} + 4 = 4 + 3\sqrt{2}$$

\subsection*{Answer}
(D) $4 + 3\sqrt{2}$

\end{document}