\documentclass[12pt]{article}
\usepackage[margin=1in]{geometry}
\usepackage{amsmath,amssymb}
\begin{document}

\section*{Problem 9}
Ako je $f(x) = \left(\frac{x + 1}{x - 1}\right)^2$ $(x \neq \pm 1)$ tada je $f\left(\frac{x + 1}{x - 1}\right) - f\left(\frac{x - 1}{x + 1}\right)$ jednako:

(A) $\left(\frac{x + 1}{x - 1}\right)^2$ \quad (B) $\left(\frac{x - 1}{x + 1}\right)^2$ \quad (C) $0$ \quad (D) $\frac{x^2 - 1}{x^2 + 1}$ \quad (E) $-\left(\frac{x - 1}{x + 1}\right)^2$ \quad (N) Ne znam

\subsection*{Solution}
Given $f(x) = \left(\frac{x + 1}{x - 1}\right)^2$, we need to find $f\left(\frac{x + 1}{x - 1}\right) - f\left(\frac{x - 1}{x + 1}\right)$.

First, let's calculate $f\left(\frac{x + 1}{x - 1}\right)$:

Let $u = \frac{x + 1}{x - 1}$. Then:
$$f(u) = \left(\frac{u + 1}{u - 1}\right)^2$$

We need to find $\frac{u + 1}{u - 1}$ where $u = \frac{x + 1}{x - 1}$:

$$\frac{u + 1}{u - 1} = \frac{\frac{x + 1}{x - 1} + 1}{\frac{x + 1}{x - 1} - 1}$$

For the numerator:
$$\frac{x + 1}{x - 1} + 1 = \frac{x + 1 + (x - 1)}{x - 1} = \frac{2x}{x - 1}$$

For the denominator:
$$\frac{x + 1}{x - 1} - 1 = \frac{x + 1 - (x - 1)}{x - 1} = \frac{2}{x - 1}$$

Therefore:
$$\frac{u + 1}{u - 1} = \frac{\frac{2x}{x - 1}}{\frac{2}{x - 1}} = \frac{2x}{2} = x$$

So $f\left(\frac{x + 1}{x - 1}\right) = x^2$.

Now let's calculate $f\left(\frac{x - 1}{x + 1}\right)$:

Let $v = \frac{x - 1}{x + 1}$. Then:
$$f(v) = \left(\frac{v + 1}{v - 1}\right)^2$$

We need to find $\frac{v + 1}{v - 1}$ where $v = \frac{x - 1}{x + 1}$:

For the numerator:
$$\frac{x - 1}{x + 1} + 1 = \frac{x - 1 + (x + 1)}{x + 1} = \frac{2x}{x + 1}$$

For the denominator:
$$\frac{x - 1}{x + 1} - 1 = \frac{x - 1 - (x + 1)}{x + 1} = \frac{-2}{x + 1}$$

Therefore:
$$\frac{v + 1}{v - 1} = \frac{\frac{2x}{x + 1}}{\frac{-2}{x + 1}} = \frac{2x}{-2} = -x$$

So $f\left(\frac{x - 1}{x + 1}\right) = (-x)^2 = x^2$.

Therefore:
$$f\left(\frac{x + 1}{x - 1}\right) - f\left(\frac{x - 1}{x + 1}\right) = x^2 - x^2 = 0$$

\subsection*{Answer}
(C) $0$

\end{document}