\documentclass[12pt]{article}
\usepackage[margin=1in]{geometry}
\usepackage{amsmath,amssymb}
\begin{document}

\section*{Problem 19}
Sva realna rešenja jednačine $\log_{2011}(2010x) = \log_{2010}(2011x)$ pripadaju intervalu:

(A) $\left(0, \frac{1}{2011}\right)$ \quad (B) $\left(\frac{1}{2011}, \frac{1}{2010}\right)$ \quad (C) $\left(\frac{1}{2010}, 1\right)$ \quad (D) $\left(1, \frac{2010}{2011}\right)$ \quad (E) $\left(\frac{2011}{2010}, +\infty\right)$ \quad (N) Ne znam

\subsection*{Solution}
Let's denote the equation as:
$$\log_{2011}(2010x) = \log_{2010}(2011x)$$

First, we need $2010x > 0$ and $2011x > 0$, so $x > 0$.

Using the change of base formula:
$$\frac{\ln(2010x)}{\ln(2011)} = \frac{\ln(2011x)}{\ln(2010)}$$

Cross-multiplying:
$$\ln(2010x) \cdot \ln(2010) = \ln(2011x) \cdot \ln(2011)$$

Using logarithm properties:
$$[\ln(2010) + \ln(x)] \cdot \ln(2010) = [\ln(2011) + \ln(x)] \cdot \ln(2011)$$

Expanding:
$$\ln^2(2010) + \ln(x) \cdot \ln(2010) = \ln^2(2011) + \ln(x) \cdot \ln(2011)$$

Rearranging:
$$\ln^2(2010) - \ln^2(2011) = \ln(x)[\ln(2011) - \ln(2010)]$$

$$\ln^2(2010) - \ln^2(2011) = \ln(x) \cdot \ln\left(\frac{2011}{2010}\right)$$

Using the difference of squares:
$$[\ln(2010) - \ln(2011)][\ln(2010) + \ln(2011)] = \ln(x) \cdot \ln\left(\frac{2011}{2010}\right)$$

$$-\ln\left(\frac{2011}{2010}\right) \cdot [\ln(2010) + \ln(2011)] = \ln(x) \cdot \ln\left(\frac{2011}{2010}\right)$$

Since $\ln\left(\frac{2011}{2010}\right) > 0$, we can divide both sides by it:
$$-[\ln(2010) + \ln(2011)] = \ln(x)$$

$$\ln(x) = -\ln(2010 \cdot 2011)$$

$$x = \frac{1}{2010 \cdot 2011}$$

Let's verify this is in the correct interval:
$$\frac{1}{2010 \cdot 2011} = \frac{1}{2010 \cdot 2011}$$

Since $2010 \cdot 2011 > 2011^2$, we have:
$$\frac{1}{2010 \cdot 2011} < \frac{1}{2011^2} < \frac{1}{2011}$$

And since $2010 \cdot 2011 > 2010^2$, we have:
$$\frac{1}{2010 \cdot 2011} < \frac{1}{2010^2} < \frac{1}{2010}$$

But we need to be more precise. Since $2010 < 2011$:
$$2010 \cdot 2011 > 2011 \cdot 2010 = 2010 \cdot 2011$$

Wait, let me recalculate more carefully:
$$\frac{1}{2011} = \frac{2010}{2011 \cdot 2010} = \frac{2010}{2010 \cdot 2011}$$
$$\frac{1}{2010} = \frac{2011}{2010 \cdot 2011}$$

Since $2010 < 2011$, we have $\frac{2010}{2010 \cdot 2011} < \frac{1}{2010 \cdot 2011} < \frac{2011}{2010 \cdot 2011}$.

Therefore: $\frac{1}{2011} < \frac{1}{2010 \cdot 2011} < \frac{1}{2010}$

So $x = \frac{1}{2010 \cdot 2011} \in \left(\frac{1}{2011}, \frac{1}{2010}\right)$.

\subsection*{Answer}
(B) $\left(\frac{1}{2011}, \frac{1}{2010}\right)$

\end{document}