\documentclass[12pt]{article}
\usepackage[margin=1in]{geometry}
\usepackage{amsmath,amssymb}
\begin{document}

\section*{Problem 5}
Zbir $\sin \frac{3\pi}{7} + \sin \frac{4\pi}{7}$ jednak je:

(A) $-2\sin \frac{\pi}{14}$ \quad (B) $-2\cos \frac{\pi}{14}$ \quad (C) $2\sin \frac{\pi}{14}$ \quad (D) $2\cos \frac{\pi}{7}$ \quad (E) $2\cos \frac{\pi}{14}$ \quad (N) Ne znam

\subsection*{Solution}
We use the sum-to-product formula:
$$\sin A + \sin B = 2\sin\left(\frac{A + B}{2}\right)\cos\left(\frac{A - B}{2}\right)$$

With $A = \frac{3\pi}{7}$ and $B = \frac{4\pi}{7}$:

\begin{align}
\frac{A + B}{2} &= \frac{\frac{3\pi}{7} + \frac{4\pi}{7}}{2} = \frac{\frac{7\pi}{7}}{2} = \frac{\pi}{2}\\
\frac{A - B}{2} &= \frac{\frac{3\pi}{7} - \frac{4\pi}{7}}{2} = \frac{-\frac{\pi}{7}}{2} = -\frac{\pi}{14}
\end{align}

Therefore:
\begin{align}
\sin \frac{3\pi}{7} + \sin \frac{4\pi}{7} &= 2\sin\left(\frac{\pi}{2}\right)\cos\left(-\frac{\pi}{14}\right)\\
&= 2 \cdot 1 \cdot \cos\left(-\frac{\pi}{14}\right)\\
&= 2\cos\left(-\frac{\pi}{14}\right)\\
&= 2\cos\left(\frac{\pi}{14}\right)
\end{align}

The last step uses the fact that cosine is an even function: $\cos(-x) = \cos(x)$.

\subsection*{Answer}
(E) $2\cos \frac{\pi}{14}$

\end{document}