\documentclass[12pt]{article}
\usepackage[margin=1in]{geometry}
\usepackage{amsmath,amssymb}
\begin{document}

\section*{Problem 3}
Ako su $x_1$ i $x_2$ rešenja kvadratne jednačine $x^2 + x + 1 = 0$, tada su $y_1 = ax_1 + x_2$ i $y_2 = x_1 + ax_2$, ($a \in \mathbf{R}$), rešenja kvadratne jednačine:

\subsection*{Solution}
By Vieta's formulas for $x^2 + x + 1 = 0$:
\[
x_1 + x_2 = -1, \quad x_1 x_2 = 1
\]

Now we find $y_1 + y_2$ and $y_1 y_2$:
\[
y_1 + y_2 = ax_1 + x_2 + x_1 + ax_2 = (a+1)(x_1 + x_2) = (a+1)(-1) = -(a+1)
\]

\[
y_1 y_2 = (ax_1 + x_2)(x_1 + ax_2) = ax_1^2 + a^2x_1x_2 + x_1x_2 + ax_2^2
\]
\[
= a(x_1^2 + x_2^2) + (a^2 + 1)x_1x_2
\]

We know that $x_1^2 + x_2^2 = (x_1 + x_2)^2 - 2x_1x_2 = 1 - 2 = -1$.

So:
\[
y_1 y_2 = a(-1) + (a^2 + 1)(1) = -a + a^2 + 1 = a^2 - a + 1
\]

The quadratic equation with roots $y_1, y_2$ is:
\[
y^2 - (y_1 + y_2)y + y_1 y_2 = 0
\]
\[
y^2 + (a+1)y + a^2 - a + 1 = 0
\]

Comparing with the options:
- (A) $y^2 + (a+1)y - a^2 + a + 1 = 0$ — coefficient of $y$ matches, but constant term is $-a^2 + a + 1 \neq a^2 - a + 1$
- (B) $y^2 + (a^2+1)y + 1 = 0$ — doesn't match
- (C) $y^2 + (a+1)y + a^2 - a + 1 = 0$ — matches!
- (D) $y^2 + (a^2+1)y + a^2 - a + 1 = 0$ — coefficient of $y$ doesn't match

\subsection*{Answer}
$y^2 + (a+1)y + a^2 - a + 1 = 0$ (option \textbf{C}).

\end{document}
