\documentclass[12pt]{article}
\usepackage[margin=1in]{geometry}
\usepackage{amsmath,amssymb}
\begin{document}

\section*{Problem 4}
Ako je $a > b > 0$ i $a^2 + b^2 = 6ab$, tada je $\frac{a+b}{a-b}$ jednako:

A) $-\sqrt{2}$; \quad B) $\sqrt{2}$; \quad C) $\sqrt{6}$; \quad D) $1$; \quad E) $\frac{1}{\sqrt{2}}$; \quad N) Ne znam.

\subsection*{Rešenje}
Iz uslova $a^2 + b^2 = 6ab$ izvedimo potrebne izraze.

Znamo da:
\begin{align*}
(a+b)^2 &= a^2 + 2ab + b^2 = 6ab + 2ab = 8ab\\
(a-b)^2 &= a^2 - 2ab + b^2 = 6ab - 2ab = 4ab
\end{align*}

Pošto je $a > b > 0$, imamo $a+b > 0$ i $a-b > 0$, pa:
\begin{align*}
a+b &= \sqrt{8ab} = 2\sqrt{2ab}\\
a-b &= \sqrt{4ab} = 2\sqrt{ab}
\end{align*}

Dakle:
\[
\frac{a+b}{a-b} = \frac{2\sqrt{2ab}}{2\sqrt{ab}} = \frac{\sqrt{2ab}}{\sqrt{ab}} = \sqrt{\frac{2ab}{ab}} = \sqrt{2}
\]

\subsection*{Odgovor}
$\sqrt{2}$ (opcija \textbf{B}).

\end{document}
