\documentclass[12pt]{article}
\usepackage[margin=1in]{geometry}
\usepackage{amsmath,amssymb}
\usepackage[utf8]{inputenc}
\begin{document}

\section*{Problem 12}
If $f(x) - 2f\left(\frac{1}{x}\right) = x^2$, $x \neq 0$, find $f(2)$.

\subsection*{Solution}
We have the equation
\[
f(x) - 2f\left(\frac{1}{x}\right) = x^2. \quad (*).
\]
Substitute $\frac{1}{x}$ for $x$ in $(*)$:
\[
f\left(\frac{1}{x}\right) - 2f(x) = \left(\frac{1}{x}\right)^2 = \frac{1}{x^2}. \quad (**).
\]
We want to find $f(2)$, so let's set $x=2$.
From $(*)$:
\[
f(2) - 2f(1/2) = 4. \quad (1)
\]
From $(**)$ with $x=2$ (or substituting $x=1/2$ into original):
\[
f(1/2) - 2f(2) = (1/2)^2 = \frac{1}{4}. \quad (2)
\]
From $(2)$, $f(1/2) = \frac{1}{4} + 2f(2)$. Substitute this into $(1)$:
\[
f(2) - 2\left(\frac{1}{4} + 2f(2)\right) = 4
\]
\[
f(2) - \frac{1}{2} - 4f(2) = 4
\]
\[
-3f(2) = 4 + \frac{1}{2} = \frac{9}{2}
\]
\[
f(2) = \frac{9/2}{-3} = -\frac{3}{2}.
\]

\subsection*{Answer}
$-\frac{3}{2}$ (option \textbf{Ð”}).

\end{document}






