\documentclass[12pt]{article}
\usepackage[margin=1in]{geometry}
\usepackage{amsmath,amssymb}
\begin{document}

\section*{Problem 19}
Ukupan broj realnih rešenja sistema $50\left(\dfrac{2}{5}\right)^{2x+3y-10} + 20\left(\dfrac{5}{2}\right)^{2x+3y-10} = 133$, $(x+3)(y-1) = 6$ jednak je:

\subsection*{Solution}
Let $t = 2x + 3y - 10$ and let $u = \left(\frac{2}{5}\right)^t$.

Then $\left(\frac{5}{2}\right)^t = \frac{1}{u}$.

The first equation becomes:
\[
50u + \frac{20}{u} = 133
\]
\[
50u^2 + 20 = 133u
\]
\[
50u^2 - 133u + 20 = 0
\]

Using the quadratic formula:
\[
u = \frac{133 \pm \sqrt{133^2 - 4 \cdot 50 \cdot 20}}{100} = \frac{133 \pm \sqrt{17689 - 4000}}{100} = \frac{133 \pm \sqrt{13689}}{100} = \frac{133 \pm 117}{100}
\]

$u_1 = \frac{250}{100} = \frac{5}{2}$ and $u_2 = \frac{16}{100} = \frac{4}{25}$

\textbf{For $u_1 = \frac{5}{2}$:}
$\left(\frac{2}{5}\right)^t = \frac{5}{2} = \left(\frac{2}{5}\right)^{-1}$
$t = -1$, so $2x + 3y = 9$

\textbf{For $u_2 = \frac{4}{25} = \left(\frac{2}{5}\right)^2$:}
$t = 2$, so $2x + 3y = 12$

Now solve with the second equation $(x+3)(y-1) = 6$.

\textbf{Case 1:} $2x + 3y = 9$ and $(x+3)(y-1) = 6$

From first: $x = \frac{9 - 3y}{2}$

Substituting: $\left(\frac{9 - 3y}{2} + 3\right)(y - 1) = 6$
$\left(\frac{15 - 3y}{2}\right)(y - 1) = 6$
$(15 - 3y)(y - 1) = 12$
$15y - 15 - 3y^2 + 3y = 12$
$-3y^2 + 18y - 27 = 0$
$y^2 - 6y + 9 = 0$
$(y - 3)^2 = 0$
$y = 3$, $x = \frac{9 - 9}{2} = 0$

One solution: $(0, 3)$

\textbf{Case 2:} $2x + 3y = 12$ and $(x+3)(y-1) = 6$

From first: $x = \frac{12 - 3y}{2}$

Substituting: $\left(\frac{12 - 3y}{2} + 3\right)(y - 1) = 6$
$\left(\frac{18 - 3y}{2}\right)(y - 1) = 6$
$(18 - 3y)(y - 1) = 12$
$18y - 18 - 3y^2 + 3y = 12$
$-3y^2 + 21y - 30 = 0$
$y^2 - 7y + 10 = 0$
$(y - 2)(y - 5) = 0$
$y = 2$ or $y = 5$

$y = 2$: $x = \frac{12 - 6}{2} = 3$ → $(3, 2)$
$y = 5$: $x = \frac{12 - 15}{2} = -\frac{3}{2}$ → $(-\frac{3}{2}, 5)$

Two solutions.

\textbf{Total:} $1 + 2 = 3$ solutions.

\subsection*{Answer}
$3$ (option \textbf{D}).

\end{document}
