\documentclass[12pt]{article}
\usepackage[margin=1in]{geometry}
\usepackage{amsmath,amssymb}
\begin{document}

\section*{Problem 9}
Ako je $f(x) = \dfrac{4}{x-5} + (3x+1)e^{-(x-1)^2} + \sqrt{-2x+3}$, tada je $f'(1)$ jednako:

\subsection*{Solution}
Let's find $f'(x)$ by differentiating each term.

\textbf{First term:} $\dfrac{4}{x-5} = 4(x-5)^{-1}$
\[
\frac{d}{dx}\left(\frac{4}{x-5}\right) = -4(x-5)^{-2} = -\frac{4}{(x-5)^2}
\]
At $x = 1$: $-\dfrac{4}{(-4)^2} = -\dfrac{4}{16} = -\dfrac{1}{4}$

\textbf{Second term:} $(3x+1)e^{-(x-1)^2}$

Using the product rule:
\[
\frac{d}{dx}\left[(3x+1)e^{-(x-1)^2}\right] = 3e^{-(x-1)^2} + (3x+1) \cdot e^{-(x-1)^2} \cdot (-2(x-1))
\]
\[
= e^{-(x-1)^2}\left[3 - 2(x-1)(3x+1)\right]
\]

At $x = 1$: $e^{0}\left[3 - 2(0)(4)\right] = 1 \cdot 3 = 3$

\textbf{Third term:} $\sqrt{-2x+3} = (-2x+3)^{1/2}$
\[
\frac{d}{dx}\sqrt{-2x+3} = \frac{1}{2}(-2x+3)^{-1/2} \cdot (-2) = \frac{-1}{\sqrt{-2x+3}}
\]
At $x = 1$: $\dfrac{-1}{\sqrt{-2+3}} = \dfrac{-1}{\sqrt{1}} = -1$

\textbf{Total:}
\[
f'(1) = -\frac{1}{4} + 3 + (-1) = -\frac{1}{4} + 2 = \frac{-1 + 8}{4} = \frac{7}{4}
\]

\subsection*{Answer}
$\dfrac{7}{4}$ (option \textbf{E}).

\end{document}
