\documentclass[12pt]{article}
\usepackage[margin=1in]{geometry}
\usepackage{amsmath,amssymb}
\begin{document}

\section*{Problem 4}
Izraz $\left(\dfrac{x\sqrt{x} - y\sqrt{y}}{\sqrt{x} - \sqrt{y}} + \sqrt{xy}\right) : \left(\dfrac{\sqrt{x} - \sqrt{y}}{x - y}\right)^{-2}$, za sve vrednosti $x, y \in \mathbb{R}$ za koje je definisan, identiƒçki je jednak izrazu:

\subsection*{Solution}
Let's simplify step by step. Let $a = \sqrt{x}$ and $b = \sqrt{y}$, so $x = a^2$ and $y = b^2$.

\textbf{First part:} $\dfrac{x\sqrt{x} - y\sqrt{y}}{\sqrt{x} - \sqrt{y}} = \dfrac{a^3 - b^3}{a - b}$

Using the factorization $a^3 - b^3 = (a-b)(a^2 + ab + b^2)$:
\[
\dfrac{a^3 - b^3}{a - b} = a^2 + ab + b^2 = x + \sqrt{xy} + y
\]

So the expression in the first parenthesis becomes:
\[
x + \sqrt{xy} + y + \sqrt{xy} = x + 2\sqrt{xy} + y = (\sqrt{x} + \sqrt{y})^2
\]

\textbf{Second part:} $\left(\dfrac{\sqrt{x} - \sqrt{y}}{x - y}\right)^{-2}$

Note that $x - y = (\sqrt{x} - \sqrt{y})(\sqrt{x} + \sqrt{y})$, so:
\[
\dfrac{\sqrt{x} - \sqrt{y}}{x - y} = \dfrac{\sqrt{x} - \sqrt{y}}{(\sqrt{x} - \sqrt{y})(\sqrt{x} + \sqrt{y})} = \dfrac{1}{\sqrt{x} + \sqrt{y}}
\]

Therefore:
\[
\left(\dfrac{1}{\sqrt{x} + \sqrt{y}}\right)^{-2} = (\sqrt{x} + \sqrt{y})^2
\]

\textbf{Final calculation:}
\[
(\sqrt{x} + \sqrt{y})^2 : (\sqrt{x} + \sqrt{y})^2 = 1
\]

\subsection*{Answer}
$1$ (option \textbf{A}).

\end{document}
