\documentclass[12pt]{article}
\usepackage[margin=1in]{geometry}
\usepackage{amsmath,amssymb}
\begin{document}

\section*{Problem 6}
Date su funkcije: $f_1(x) = \ln((x+3)^5 \cdot (x-1)^2)$, $f_2(x) = 5\ln(x+3) + \ln(x-1)^2$, $f_3(x) = \ln(x+3)^5 + 2\ln(x-1)$ i $f_4(x) = 5\ln(x+3) + 2\ln(x-1)$. TaÄan iskaz je:

\subsection*{Solution}
Let's analyze the domains and expressions of each function.

\textbf{$f_1(x) = \ln((x+3)^5 \cdot (x-1)^2)$}

For this to be defined, we need $(x+3)^5 \cdot (x-1)^2 > 0$.
- $(x-1)^2 \geq 0$ always, and $= 0$ when $x = 1$
- $(x+3)^5 > 0$ when $x > -3$, and $< 0$ when $x < -3$

So we need $x > -3$ and $x \neq 1$. Domain: $(-3, 1) \cup (1, +\infty)$

\textbf{$f_2(x) = 5\ln(x+3) + \ln(x-1)^2$}

We need $x + 3 > 0$ and $(x-1)^2 > 0$.
This gives $x > -3$ and $x \neq 1$. Domain: $(-3, 1) \cup (1, +\infty)$

Note: $\ln(x-1)^2 = 2\ln|x-1|$

\textbf{$f_3(x) = \ln(x+3)^5 + 2\ln(x-1)$}

We need $x + 3 > 0$ and $x - 1 > 0$.
This gives $x > 1$. Domain: $(1, +\infty)$

\textbf{$f_4(x) = 5\ln(x+3) + 2\ln(x-1)$}

We need $x + 3 > 0$ and $x - 1 > 0$.
This gives $x > 1$. Domain: $(1, +\infty)$

For $x > 1$, all functions are defined. Let's check if they're equal there:
- $f_1(x) = \ln((x+3)^5) + \ln((x-1)^2) = 5\ln(x+3) + 2\ln(x-1)$
- $f_2(x) = 5\ln(x+3) + 2\ln|x-1| = 5\ln(x+3) + 2\ln(x-1)$ for $x > 1$
- $f_3(x) = 5\ln(x+3) + 2\ln(x-1)$
- $f_4(x) = 5\ln(x+3) + 2\ln(x-1)$

On $(1, +\infty)$: $f_1 = f_2 = f_3 = f_4$

But $f_3$ and $f_4$ have domain $(1, +\infty)$, while $f_1$ and $f_2$ have domain $(-3, 1) \cup (1, +\infty)$.

So $f_1 = f_2$ (same domain and same values), but $f_1 \neq f_3$ and $f_1 \neq f_4$ (different domains).

Also $f_3 = f_4$ on their common domain.

Therefore: $f_1 = f_2 \neq f_3 = f_4$

\subsection*{Answer}
$f_1 = f_2 \neq f_3 = f_4$ (option \textbf{D}).

\end{document}
