\documentclass[12pt]{article}
\usepackage[margin=1in]{geometry}
\usepackage{amsmath,amssymb}
\begin{document}

\section*{Problem 17}
Ako je rešenje jednačine
\[
4^{x+\sqrt{x^2-2}}-5\cdot 2^{x-1+\sqrt{x^2-2}}=6
\]
oblika $\dfrac{p}{q}$, tada je $p+q$ jednako:
\[
\text{(A) }-3\quad \text{(B) }4\quad \text{(C) }5\quad \text{(D) }-5\quad \text{(E) }-4\quad \text{(N) Ne znam.}
\]

\subsection*{Solution}
Označimo
\[
t=2^{x+\sqrt{x^2-2}} \quad (>0).
\]
Tada je
\[
4^{x+\sqrt{x^2-2}}=\left(2^2\right)^{x+\sqrt{x^2-2}}=2^{2(x+\sqrt{x^2-2})}=t^2,
\]
a
\[
2^{x-1+\sqrt{x^2-2}}=2^{-1}\cdot 2^{x+\sqrt{x^2-2}}=\frac{t}{2}.
\]
Jednačina postaje
\[
t^2-5\cdot\frac{t}{2}=6 \;\Longleftrightarrow\; 2t^2-5t-12=0.
\]
Rešenja su
\[
t=\frac{5\pm \sqrt{25+96}}{4}=\frac{5\pm 11}{4}\in\left\{4,-\frac{3}{2}\right\}.
\]
Pošto je $t>0$, sledi $t=4$, odnosno
\[
2^{x+\sqrt{x^2-2}}=4=2^2 \Rightarrow x+\sqrt{x^2-2}=2.
\]
Zato je $\sqrt{x^2-2}=2-x$ (pa $x\le 2$). Kvadriranjem:
\[
x^2-2=(2-x)^2=x^2-4x+4 \Rightarrow -2=-4x+4 \Rightarrow x=\frac{3}{2}.
\]
Dakle, $x=\frac{p}{q}=\frac{3}{2}$ pa je $p+q=3+2=5$.

\subsection*{Answer}
$5$ (option \textbf{C}).

\end{document}

