\documentclass[12pt]{article}
\usepackage[margin=1in]{geometry}
\usepackage{amsmath,amssymb}
\begin{document}

\section*{Problem 10}
Ako je $f(x) = 2x + |x|$ i $g(x) = \frac{2}{3}x - \frac{1}{3}|x|$, tada je $f(g(x))$ jednako:

\subsection*{Solution}
Prvo analiziramo funkciju $g(x) = \frac{2}{3}x - \frac{1}{3}|x|$.

Za $x \geq 0$: $|x| = x$, pa je $g(x) = \frac{2}{3}x - \frac{1}{3}x = \frac{1}{3}x \geq 0$.

Za $x < 0$: $|x| = -x$, pa je $g(x) = \frac{2}{3}x - \frac{1}{3}(-x) = \frac{2}{3}x + \frac{1}{3}x = x < 0$.

Dakle:
\[
g(x) = \begin{cases}
\frac{1}{3}x & \text{ako } x \geq 0 \\
x & \text{ako } x < 0
\end{cases}
\]

Sada raÄunamo $f(g(x))$ gde je $f(x) = 2x + |x|$.

Za $x \geq 0$: $g(x) = \frac{1}{3}x \geq 0$, pa je:
\[
f(g(x)) = f\left(\frac{1}{3}x\right) = 2 \cdot \frac{1}{3}x + \left|\frac{1}{3}x\right| = \frac{2}{3}x + \frac{1}{3}x = x
\]

Za $x < 0$: $g(x) = x < 0$, pa je:
\[
f(g(x)) = f(x) = 2x + |x| = 2x + (-x) = x
\]

Dakle, $f(g(x)) = x$ za sve $x$.

\subsection*{Answer}
$x$ (option \textbf{D}).

\end{document}