\documentclass[12pt]{article}
\usepackage[margin=1in]{geometry}
\usepackage{amsmath,amssymb}
\begin{document}

\section*{Problem 6}
Ako je $\frac{\cos(\alpha + \beta)}{\cos(\alpha - \beta)} = \frac{1}{3}$ ($\alpha, \beta \neq \frac{\pi}{2} + k\pi$, $\alpha - \beta \neq \frac{\pi}{2} + m\pi$, $k, m \in \mathbb{Z}$), tada je $\text{tg}\alpha \cdot \text{tg}\beta$ jednako:

\subsection*{Solution}
Koristimo formule za kosinus zbira i razlike:
\[
\cos(\alpha + \beta) = \cos\alpha\cos\beta - \sin\alpha\sin\beta
\]
\[
\cos(\alpha - \beta) = \cos\alpha\cos\beta + \sin\alpha\sin\beta
\]

Iz datog uslova:
\[
\frac{\cos\alpha\cos\beta - \sin\alpha\sin\beta}{\cos\alpha\cos\beta + \sin\alpha\sin\beta} = \frac{1}{3}
\]

Krstno mno≈æenje:
\[
3(\cos\alpha\cos\beta - \sin\alpha\sin\beta) = \cos\alpha\cos\beta + \sin\alpha\sin\beta
\]
\[
3\cos\alpha\cos\beta - 3\sin\alpha\sin\beta = \cos\alpha\cos\beta + \sin\alpha\sin\beta
\]
\[
2\cos\alpha\cos\beta = 4\sin\alpha\sin\beta
\]
\[
\frac{\sin\alpha\sin\beta}{\cos\alpha\cos\beta} = \frac{2}{4} = \frac{1}{2}
\]
\[
\text{tg}\alpha \cdot \text{tg}\beta = \frac{1}{2}
\]

\subsection*{Answer}
$\frac{1}{2}$ (option \textbf{B}).

\end{document}