\documentclass[12pt]{article}
\usepackage[margin=1in]{geometry}
\usepackage{amsmath,amssymb}
\begin{document}

\section*{Problem 11}
Proizvod svih realnih rešenja jednačine $\displaystyle\frac{2013x}{2014} = 2013^{\log_x 2014}$ pripada skupu:

(A) $(0, 1]$ \quad (B) $(1, 2]$ \quad (C) $(2, 3]$ \quad (D) $(3, 4]$ \quad (E) $(4, +\infty)$ \quad (N) Ne znam

\subsection*{Solution}
Let $y = \log_x 2014$, which means $x^y = 2014$.

The equation becomes:
\[
\frac{2013x}{2014} = 2013^y
\]

Taking logarithm base 2013:
\[
\log_{2013}\left(\frac{2013x}{2014}\right) = y
\]
\[
\log_{2013}(2013x) - \log_{2013}(2014) = y
\]
\[
1 + \log_{2013}x - \log_{2013}(2014) = y
\]

Since $y = \log_x 2014 = \frac{\ln 2014}{\ln x}$, and $\log_{2013} x = \frac{\ln x}{\ln 2013}$.

Let $a = \ln x$ and $b = \ln 2013$, $c = \ln 2014$.

Then $y = \frac{c}{a}$ and the equation becomes:
\[
1 + \frac{a}{b} - \frac{c}{b} = \frac{c}{a}
\]
\[
\frac{b + a - c}{b} = \frac{c}{a}
\]
\[
a(b + a - c) = bc
\]
\[
a^2 + ab - ac - bc = 0
\]
\[
a^2 + a(b-c) - bc = 0
\]

Using the quadratic formula with $a$ as variable:
\[
a = \frac{-(b-c) \pm \sqrt{(b-c)^2 + 4bc}}{2} = \frac{(c-b) \pm \sqrt{(b-c)^2 + 4bc}}{2}
\]

Note that $(b-c)^2 + 4bc = b^2 - 2bc + c^2 + 4bc = b^2 + 2bc + c^2 = (b+c)^2$.

So:
\[
a = \frac{(c-b) \pm (b+c)}{2}
\]

This gives $a_1 = \frac{c-b+b+c}{2} = c$ and $a_2 = \frac{c-b-b-c}{2} = -b$.

So $\ln x_1 = c = \ln 2014 \implies x_1 = 2014$

And $\ln x_2 = -b = -\ln 2013 \implies x_2 = \frac{1}{2013}$

The product of solutions:
\[
x_1 \cdot x_2 = 2014 \cdot \frac{1}{2013} = \frac{2014}{2013} \approx 1.0005
\]

Since $\frac{2014}{2013} > 1$ and $\frac{2014}{2013} < 2$, the product belongs to $(1, 2]$.

\subsection*{Answer}
$(1, 2]$ (option \textbf{B}).

\end{document}
