\documentclass[12pt]{article}
\usepackage[margin=1in]{geometry}
\usepackage{amsmath,amssymb}
\begin{document}

\section*{Problem 6}
Ako je $f\left(\frac{1-x}{1+x}\right) = x$ $(x \in \mathbf{R} \setminus \{-1, 0, 1\})$, tada je $f(f(x))$ jednako:

(A) $x$ \quad (B) $\displaystyle\frac{1-x}{1+x}$ \quad (C) $\displaystyle\frac{1}{x}$ \quad (D) $\displaystyle\frac{1+x}{1-x}$ \quad (E) $2x$ \quad (N) Ne znam

\subsection*{Solution}
Given $f\left(\frac{1-x}{1+x}\right) = x$.

Let $t = \frac{1-x}{1+x}$. We need to express $x$ in terms of $t$:
\[
t(1+x) = 1-x \implies t + tx = 1 - x \implies tx + x = 1 - t \implies x(t+1) = 1-t
\]
\[
x = \frac{1-t}{1+t}
\]

Therefore:
\[
f(t) = \frac{1-t}{1+t}
\]

Now we compute $f(f(x))$:
\[
f(x) = \frac{1-x}{1+x}
\]

\[
f(f(x)) = f\left(\frac{1-x}{1+x}\right) = \frac{1 - \frac{1-x}{1+x}}{1 + \frac{1-x}{1+x}}
\]

Simplifying the numerator:
\[
1 - \frac{1-x}{1+x} = \frac{(1+x) - (1-x)}{1+x} = \frac{2x}{1+x}
\]

Simplifying the denominator:
\[
1 + \frac{1-x}{1+x} = \frac{(1+x) + (1-x)}{1+x} = \frac{2}{1+x}
\]

Therefore:
\[
f(f(x)) = \frac{\frac{2x}{1+x}}{\frac{2}{1+x}} = \frac{2x}{2} = x
\]

\subsection*{Answer}
$x$ (option \textbf{A}).

\end{document}
