\documentclass[12pt]{article}
\usepackage[margin=1in]{geometry}
\usepackage{amsmath,amssymb}
\begin{document}

\section*{Problem 9}
Data je kvadratna funkcija $f(x) = x^2 + bx + c$ $(b, c \in \mathbf{R})$ takva da je $f(f(1)) = f(f(2)) = 0$, pri ƒçemu je $f(1) \neq f(2)$. Vrednost $f(0)$ jednaka je:

(A) $-6$ \quad (B) $-\frac{2}{3}$ \quad (C) $-\frac{3}{2}$ \quad (D) $-\frac{1}{4}$ \quad (E) $-2$ \quad (N) Ne znam

\subsection*{Solution}
Let $f(1) = u$ and $f(2) = v$ where $u \neq v$.

Since $f(f(1)) = f(u) = 0$ and $f(f(2)) = f(v) = 0$, both $u$ and $v$ are roots of $f(x) = 0$.

So $f(x) = (x - u)(x - v) = x^2 - (u+v)x + uv$.

Comparing with $f(x) = x^2 + bx + c$:
\[
b = -(u+v), \quad c = uv
\]

Now compute $f(1)$ and $f(2)$:
\[
f(1) = 1 + b + c = u
\]
\[
f(2) = 4 + 2b + c = v
\]

From these:
\[
1 + b + c = u \implies 1 - (u+v) + uv = u \implies 1 - u - v + uv = u
\]
\[
1 - v + uv = 2u \implies 1 - v(1-u) = 2u \quad (1)
\]

\[
4 + 2b + c = v \implies 4 - 2(u+v) + uv = v
\]
\[
4 - 2u - 2v + uv = v \implies 4 - 2u + uv = 3v \quad (2)
\]

From equation (1): $1 + uv - v = 2u$, so $uv = 2u + v - 1$.

Substituting into equation (2):
\[
4 - 2u + (2u + v - 1) = 3v
\]
\[
4 - 2u + 2u + v - 1 = 3v
\]
\[
3 + v = 3v \implies 3 = 2v \implies v = \frac{3}{2}
\]

From $uv = 2u + v - 1$:
\[
u \cdot \frac{3}{2} = 2u + \frac{3}{2} - 1
\]
\[
\frac{3u}{2} = 2u + \frac{1}{2}
\]
\[
3u = 4u + 1 \implies -u = 1 \implies u = -1
\]

Therefore:
\[
c = uv = (-1) \cdot \frac{3}{2} = -\frac{3}{2}
\]

And $f(0) = c = -\frac{3}{2}$.

\subsection*{Answer}
$-\frac{3}{2}$ (option \textbf{C}).

\end{document}
