\documentclass[12pt]{article}
\usepackage[margin=1in]{geometry}
\usepackage{amsmath,amssymb}
\usepackage[utf8]{inputenc}
\begin{document}

\section*{Problem 16}
U razvoju stepena binoma $(\sqrt{x} - \frac{1}{\sqrt[3]{x}})^8$ jedan ƒçlan je $a \cdot x^{-1/6}$. Tada je $a$ jednako:
\begin{itemize}
    \item[A)] $0$
    \item[B)] $56$
    \item[C)] $-56$
    \item[D)] $-70$
    \item[E)] $70$
    \item[N)] Ne znam
\end{itemize}

\subsection*{Solution}
The general term in the expansion of $(A + B)^n$ is given by $T_{k+1} = \binom{n}{k} A^{n-k} B^k$.
Here $n=8$, $A = \sqrt{x} = x^{1/2}$, and $B = -x^{-1/3}$.
\[ T_{k+1} = \binom{8}{k} (x^{1/2})^{8-k} (-x^{-1/3})^k = \binom{8}{k} (-1)^k x^{\frac{8-k}{2}} x^{-\frac{k}{3}}. \]
Combine the exponents of $x$:
\[ T_{k+1} = \binom{8}{k} (-1)^k x^{\frac{8-k}{2} - \frac{k}{3}}. \]
We are given that the term is $a \cdot x^{-1/6}$. So the exponent must be $-1/6$:
\[ \frac{8-k}{2} - \frac{k}{3} = -\frac{1}{6}. \]
Multiply by 6 to clear denominators:
\[ 3(8-k) - 2k = -1. \]
\[ 24 - 3k - 2k = -1. \]
\[ 24 - 5k = -1 \implies 5k = 25 \implies k = 5. \]
Now find the coefficient $a$:
\[ a = \binom{8}{5} (-1)^5 = -\binom{8}{5}. \]
Use the property $\binom{n}{k} = \binom{n}{n-k}$:
\[ \binom{8}{5} = \binom{8}{3} = \frac{8 \cdot 7 \cdot 6}{3 \cdot 2 \cdot 1} = 56. \]
Thus, $a = -56$.

\subsection*{Answer}
The value of $a$ is $-56$, which corresponds to option \textbf{C}.

\end{document}