\documentclass[12pt]{article}
\usepackage[margin=1in]{geometry}
\usepackage{amsmath,amssymb}
\usepackage[utf8]{inputenc}
\begin{document}

\section*{Problem 8}
Ako je $\log_{b^2} x + \log_{x^2} b = 1, b>0, b \ne 1, x \ne 1$, tada je $x$ jednako:
\begin{itemize}
    \item[A)] $\frac{1}{b}$
    \item[B)] $\frac{1}{b^2}$
    \item[C)] $b$
    \item[D)] $b^2$
    \item[E)] $\sqrt{b}$
    \item[N)] Ne znam
\end{itemize}

\subsection*{Solution}
Recall the change of base formula and logarithm properties:
\[ \log_{b^2} x = \frac{\log_b x}{\log_b b^2} = \frac{\log_b x}{2}. \]
\[ \log_{x^2} b = \frac{\log_b b}{\log_b x^2} = \frac{1}{2 \log_b x}. \]
Let $t = \log_b x$. The equation becomes:
\[ \frac{t}{2} + \frac{1}{2t} = 1. \]
Multiply by $2t$ (assuming $t \neq 0$, which holds since $x \neq 1$):
\[ t^2 + 1 = 2t. \]
\[ t^2 - 2t + 1 = 0 \implies (t-1)^2 = 0 \implies t = 1. \]
Substitute back $t = \log_b x$:
\[ \log_b x = 1 \implies x = b. \]

\subsection*{Answer}
The value is $b$, which corresponds to option \textbf{C}.

\end{document}