\documentclass[12pt]{article}
\usepackage[margin=1in]{geometry}
\usepackage{amsmath,amssymb}
\usepackage[utf8]{inputenc}
\begin{document}

\section*{Problem 1}
Ako je $i$ imaginarna jedinica onda je koliƒçnik $\frac{i^{2004} + i^{2005}}{i^{2003} - i^{2002}}$ jednak:
\begin{itemize}
    \item[A)] $0$
    \item[B)] $-i$
    \item[C)] $1$
    \item[D)] $-1$
    \item[E)] $i$
    \item[N)] Ne znam
\end{itemize}

\subsection*{Solution}
We use the property that powers of $i$ cycle with period 4:
\[ i^1 = i, \quad i^2 = -1, \quad i^3 = -i, \quad i^4 = 1. \]
The exponents are:
\begin{align*}
2004 &= 4 \times 501 + 0 \implies i^{2004} = i^0 = 1 \\
2005 &= 4 \times 501 + 1 \implies i^{2005} = i^1 = i \\
2003 &= 4 \times 500 + 3 \implies i^{2003} = i^3 = -i \\
2002 &= 4 \times 500 + 2 \implies i^{2002} = i^2 = -1
\end{align*}
Substituting these values into the expression:
\[ \frac{i^{2004} + i^{2005}}{i^{2003} - i^{2002}} = \frac{1 + i}{-i - (-1)} = \frac{1 + i}{1 - i}. \]
To simplify, multiply the numerator and denominator by the conjugate of the denominator $(1+i)$:
\[ \frac{1+i}{1-i} \cdot \frac{1+i}{1+i} = \frac{(1+i)^2}{1^2 - i^2} = \frac{1 + 2i + i^2}{1 - (-1)} = \frac{1 + 2i - 1}{2} = \frac{2i}{2} = i. \]

\subsection*{Answer}
The value is $i$, which corresponds to option \textbf{E}.

\end{document}