\documentclass[12pt]{article}
\usepackage[margin=1in]{geometry}
\usepackage{amsmath,amssymb}
\usepackage[utf8]{inputenc}
\begin{document}

\section*{Problem 17}
Dati su izrazi $E_1 = \sin^2 \frac{x+y}{2} + \cos x \cos y, E_2 = \cos^2 \frac{x-y}{2} - \sin x \sin y, E_3 = \cos^2 \frac{x+y}{2} + \sin x \sin y, E_4 = \sin^2 \frac{x-y}{2} + \cos x \cos y$. Tačan je iskaz:
\begin{itemize}
    \item[A)] $E_1 \neq E_2, E_3 = E_4$
    \item[B)] $E_1 = E_2, E_3 \neq E_4$
    \item[C)] Među datim izrazima nema međusobno jednakih
    \item[D)] $E_1 = E_2, E_3 = E_4$
    \item[E)] $E_1 = E_3, E_2 = E_4$
    \item[N)] Ne znam
\end{itemize}

\subsection*{Solution}
Let's simplify $E_1$.
Recall that $\cos(x+y) = \cos x \cos y - \sin x \sin y$, so $\cos x \cos y = \cos(x+y) + \sin x \sin y$.
\[ E_1 = \sin^2 \frac{x+y}{2} + \cos(x+y) + \sin x \sin y. \]
Using the half-angle identity $\cos(x+y) = 1 - 2\sin^2 \frac{x+y}{2}$:
\[ E_1 = \sin^2 \frac{x+y}{2} + (1 - 2\sin^2 \frac{x+y}{2}) + \sin x \sin y = 1 - \sin^2 \frac{x+y}{2} + \sin x \sin y = \cos^2 \frac{x+y}{2} + \sin x \sin y. \]
We observe that this is exactly expression $E_3$. So $E_1 = E_3$.

Now let's simplify $E_4$.
Recall that $\cos(x-y) = \cos x \cos y + \sin x \sin y$, so $\cos x \cos y = \cos(x-y) - \sin x \sin y$.
\[ E_4 = \sin^2 \frac{x-y}{2} + \cos(x-y) - \sin x \sin y. \]
Using the identity $\cos(x-y) = 1 - 2\sin^2 \frac{x-y}{2}$:
\[ E_4 = \sin^2 \frac{x-y}{2} + (1 - 2\sin^2 \frac{x-y}{2}) - \sin x \sin y = 1 - \sin^2 \frac{x-y}{2} - \sin x \sin y = \cos^2 \frac{x-y}{2} - \sin x \sin y. \]
We observe that this is exactly expression $E_2$. So $E_2 = E_4$.

Thus, $E_1 = E_3$ and $E_2 = E_4$.

\subsection*{Answer}
The correct statement is $E_1 = E_3, E_2 = E_4$, which corresponds to option \textbf{E}.

\end{document}