\documentclass[12pt]{article}
\usepackage[margin=1in]{geometry}
\usepackage{amsmath,amssymb}
\begin{document}

\section*{Problem 7}
Find the first derivative of the function:
\[
f(x) = \ln\frac{x^2 - 1 + \sqrt{x^4 + 1}}{x}
\]
at the point $x_0 = 1$.

\subsection*{Solution}
First, let's rewrite the function:
\[
f(x) = \ln(x^2 - 1 + \sqrt{x^4 + 1}) - \ln x
\]

Taking the derivative:
\[
f'(x) = \frac{1}{x^2 - 1 + \sqrt{x^4 + 1}} \cdot \frac{d}{dx}(x^2 - 1 + \sqrt{x^4 + 1}) - \frac{1}{x}
\]

Now we need:
\[
\frac{d}{dx}(x^2 - 1 + \sqrt{x^4 + 1}) = 2x + \frac{1}{2\sqrt{x^4 + 1}} \cdot 4x^3 = 2x + \frac{2x^3}{\sqrt{x^4 + 1}}
\]

So:
\[
f'(x) = \frac{2x + \frac{2x^3}{\sqrt{x^4 + 1}}}{x^2 - 1 + \sqrt{x^4 + 1}} - \frac{1}{x}
\]

At $x_0 = 1$:
\[
\sqrt{1^4 + 1} = \sqrt{2}
\]

The numerator becomes:
\[
2(1) + \frac{2(1)^3}{\sqrt{2}} = 2 + \frac{2}{\sqrt{2}} = 2 + \sqrt{2}
\]

The denominator becomes:
\[
1^2 - 1 + \sqrt{2} = \sqrt{2}
\]

Therefore:
\[
f'(1) = \frac{2 + \sqrt{2}}{\sqrt{2}} - 1 = \frac{2}{\sqrt{2}} + 1 - 1 = \frac{2}{\sqrt{2}} = \sqrt{2}
\]

\subsection*{Answer}
$\sqrt{2}$ (option \textbf{D}).

\end{document}