\documentclass[12pt]{article}
\usepackage[margin=1in]{geometry}
\usepackage{amsmath,amssymb}
\begin{document}

\section*{Problem 3}
Given the complex number:
\[
z = \frac{\sqrt{2016} + i^{2019}}{\sqrt{2016} + i^{2017}}, \quad (i^2 = -1)
\]
Find the value of $\frac{z + \overline{z}}{2}$ (where $\overline{z}$ is the complex conjugate of $z$).

\subsection*{Solution}
First, let's simplify the powers of $i$:
\begin{align}
i^{2017} &= i^{4 \cdot 504 + 1} = (i^4)^{504} \cdot i = 1^{504} \cdot i = i\\
i^{2019} &= i^{4 \cdot 504 + 3} = (i^4)^{504} \cdot i^3 = 1^{504} \cdot (-i) = -i
\end{align}

So our expression becomes:
\[
z = \frac{\sqrt{2016} + (-i)}{\sqrt{2016} + i} = \frac{\sqrt{2016} - i}{\sqrt{2016} + i}
\]

To find $z$, we multiply numerator and denominator by the conjugate of the denominator:
\[
z = \frac{\sqrt{2016} - i}{\sqrt{2016} + i} \cdot \frac{\sqrt{2016} - i}{\sqrt{2016} - i} = \frac{(\sqrt{2016} - i)^2}{(\sqrt{2016})^2 - (i)^2}
\]

\[
= \frac{2016 - 2\sqrt{2016}i + i^2}{2016 - (-1)} = \frac{2016 - 2\sqrt{2016}i - 1}{2017} = \frac{2015 - 2\sqrt{2016}i}{2017}
\]

Therefore:
\[
z = \frac{2015}{2017} - \frac{2\sqrt{2016}}{2017}i
\]

The complex conjugate is:
\[
\overline{z} = \frac{2015}{2017} + \frac{2\sqrt{2016}}{2017}i
\]

Finally:
\[
\frac{z + \overline{z}}{2} = \frac{1}{2}\left(\frac{2015}{2017} - \frac{2\sqrt{2016}}{2017}i + \frac{2015}{2017} + \frac{2\sqrt{2016}}{2017}i\right) = \frac{2015}{2017}
\]

Since $\frac{2015}{2017} = \frac{2016-1}{2016+1} = \frac{2016-1}{2017}$, this equals $\frac{2015}{2017}$.

\subsection*{Answer}
$\frac{2015}{2017}$ (option \textbf{C}).

\end{document}