\documentclass[12pt]{article}
\usepackage[margin=1in]{geometry}
\usepackage{amsmath,amssymb}
\begin{document}

\section*{Problem 13}
If the polynomial $x^{2016} + x^{2015} - x^{2014} + ax^{2013} - bx^2 + c$ (where $a,b,c \in \mathbb{R}$) is divisible by polynomial $x^3 - x$, find $4a^2 + 3b^2 + 8c^2$.

\subsection*{Solution}
Since the polynomial is divisible by $x^3 - x = x(x^2 - 1) = x(x-1)(x+1)$, it must have roots at $x = 0, 1, -1$.

Let $P(x) = x^{2016} + x^{2015} - x^{2014} + ax^{2013} - bx^2 + c$.

From $P(0) = 0$:
\[
0^{2016} + 0^{2015} - 0^{2014} + a \cdot 0^{2013} - b \cdot 0^2 + c = 0
\]
\[
c = 0
\]

From $P(1) = 0$:
\[
1^{2016} + 1^{2015} - 1^{2014} + a \cdot 1^{2013} - b \cdot 1^2 + c = 0
\]
\[
1 + 1 - 1 + a - b + 0 = 0
\]
\[
1 + a - b = 0 \Rightarrow a - b = -1
\]

From $P(-1) = 0$:
\[
(-1)^{2016} + (-1)^{2015} - (-1)^{2014} + a(-1)^{2013} - b(-1)^2 + c = 0
\]

Since 2016, 2014 are even and 2015, 2013 are odd:
\[
1 + (-1) - 1 + a(-1) - b \cdot 1 + 0 = 0
\]
\[
1 - 1 - 1 - a - b = 0
\]
\[
-1 - a - b = 0 \Rightarrow a + b = -1
\]

Now we have the system:
\begin{align}
a - b &= -1\\
a + b &= -1
\end{align}

Adding the equations: $2a = -2 \Rightarrow a = -1$

Subtracting the first from the second: $2b = 0 \Rightarrow b = 0$

Therefore: $a = -1$, $b = 0$, $c = 0$.

Finally:
\[
4a^2 + 3b^2 + 8c^2 = 4(-1)^2 + 3(0)^2 + 8(0)^2 = 4 + 0 + 0 = 4
\]

\subsection*{Answer}
4 (option \textbf{A}).

\end{document}