\documentclass[12pt]{article}
\usepackage[margin=1in]{geometry}
\usepackage{amsmath,amssymb}
\begin{document}

\section*{Problem 5}
In an arithmetic progression of 11 terms, the first, fifth and eleventh terms form a geometric progression. If the first term of the arithmetic progression is 24, find the sum of all terms of the arithmetic progression.

\subsection*{Solution}
Let the arithmetic progression be: $a_1, a_2, \ldots, a_{11}$ where $a_1 = 24$ and common difference is $d$.

The terms are:
\begin{align}
a_1 &= 24\\
a_5 &= a_1 + 4d = 24 + 4d\\
a_{11} &= a_1 + 10d = 24 + 10d
\end{align}

Since $a_1, a_5, a_{11}$ form a geometric progression, we have:
\[
\frac{a_5}{a_1} = \frac{a_{11}}{a_5}
\]

This gives us:
\[
a_5^2 = a_1 \cdot a_{11}
\]

Substituting:
\[
(24 + 4d)^2 = 24 \cdot (24 + 10d)
\]

Expanding the left side:
\[
576 + 192d + 16d^2 = 576 + 240d
\]

Simplifying:
\[
192d + 16d^2 = 240d
\]
\[
16d^2 - 48d = 0
\]
\[
16d(d - 3) = 0
\]

So $d = 0$ or $d = 3$.

If $d = 0$, all terms are equal to 24, and $a_1 = a_5 = a_{11} = 24$ forms a geometric progression with ratio 1.

If $d = 3$, then $a_1 = 24$, $a_5 = 36$, $a_{11} = 54$. Check: $\frac{36}{24} = \frac{3}{2}$ and $\frac{54}{36} = \frac{3}{2}$, so this is also a geometric progression.

For the sum of arithmetic progression:
\[
S_n = \frac{n}{2}(2a_1 + (n-1)d) = \frac{11}{2}(2 \cdot 24 + 10d) = \frac{11}{2}(48 + 10d)
\]

Case 1: $d = 0$: $S_{11} = \frac{11}{2} \cdot 48 = 264$

Case 2: $d = 3$: $S_{11} = \frac{11}{2}(48 + 30) = \frac{11}{2} \cdot 78 = 429$

Since 429 appears in the options, the answer is 429.

\subsection*{Answer}
429 (option \textbf{D}).

\end{document}