\documentclass[12pt]{article}
\usepackage[margin=1in]{geometry}
\usepackage{amsmath,amssymb}
\begin{document}

\section*{Problem 18}
Find the sum of all real solutions to the equation:
\[
2\sqrt{x} \cdot 4^x + 5 \cdot 2^{x+1} + 2\sqrt{x} = 2^{2x+2} + 5\sqrt{x} \cdot 2^x + 4
\]

\subsection*{Solution}
First, let's rewrite the equation using the fact that $4^x = (2^2)^x = 2^{2x}$ and $2^{x+1} = 2 \cdot 2^x$ and $2^{2x+2} = 4 \cdot 2^{2x}$:

\[
2\sqrt{x} \cdot 2^{2x} + 5 \cdot 2 \cdot 2^x + 2\sqrt{x} = 4 \cdot 2^{2x} + 5\sqrt{x} \cdot 2^x + 4
\]

\[
2\sqrt{x} \cdot 2^{2x} + 10 \cdot 2^x + 2\sqrt{x} = 4 \cdot 2^{2x} + 5\sqrt{x} \cdot 2^x + 4
\]

Rearranging:
\[
2\sqrt{x} \cdot 2^{2x} - 4 \cdot 2^{2x} + 10 \cdot 2^x - 5\sqrt{x} \cdot 2^x + 2\sqrt{x} - 4 = 0
\]

Factor:
\[
2^{2x}(2\sqrt{x} - 4) + 2^x(10 - 5\sqrt{x}) + (2\sqrt{x} - 4) = 0
\]

\[
(2\sqrt{x} - 4)(2^{2x} + 1) + 5 \cdot 2^x(2 - \sqrt{x}) = 0
\]

\[
(2\sqrt{x} - 4)(2^{2x} + 1) - 5 \cdot 2^x(\sqrt{x} - 2) = 0
\]

Note that $2\sqrt{x} - 4 = 2(\sqrt{x} - 2)$, so:
\[
2(\sqrt{x} - 2)(2^{2x} + 1) - 5 \cdot 2^x(\sqrt{x} - 2) = 0
\]

\[
(\sqrt{x} - 2)[2(2^{2x} + 1) - 5 \cdot 2^x] = 0
\]

\[
(\sqrt{x} - 2)[2 \cdot 2^{2x} + 2 - 5 \cdot 2^x] = 0
\]

\[
(\sqrt{x} - 2)[2^{2x+1} - 5 \cdot 2^x + 2] = 0
\]

This gives us two cases:

Case 1: $\sqrt{x} - 2 = 0 \Rightarrow \sqrt{x} = 2 \Rightarrow x = 4$

Case 2: $2^{2x+1} - 5 \cdot 2^x + 2 = 0$

For Case 2, let $y = 2^x$. Then $2^{2x} = y^2$ and the equation becomes:
\[
2y^2 - 5y + 2 = 0
\]

Using the quadratic formula:
\[
y = \frac{5 \pm \sqrt{25 - 16}}{4} = \frac{5 \pm 3}{4}
\]

So $y = 2$ or $y = \frac{1}{2}$.

If $y = 2$: $2^x = 2 \Rightarrow x = 1$
If $y = \frac{1}{2}$: $2^x = \frac{1}{2} = 2^{-1} \Rightarrow x = -1$

Since we need $x \geq 0$ for $\sqrt{x}$ to be real, we discard $x = -1$.

Therefore, the real solutions are $x = 1$ and $x = 4$.

The sum of all real solutions is $1 + 4 = 5$.

\subsection*{Answer}
5 (option \textbf{A}).

\end{document}