\documentclass[12pt]{article}
\usepackage[margin=1in]{geometry}
\usepackage{amsmath,amssymb}
\begin{document}

\section*{Problem 16}
In the binomial expansion of $(x+y)^n$ where $x, y \in \mathbf{R}$, $n \in \mathbf{N}$, the second term equals 240, the third term equals 720, and the fourth term equals 1080. Find the sum $x + y + n$.

\subsection*{Solution}
The general term in the expansion of $(x+y)^n$ is:
\[
T_{k+1} = \binom{n}{k} x^{n-k} y^k
\]

So:
\begin{align*}
T_2 &= \binom{n}{1} x^{n-1} y = nx^{n-1}y = 240 \\
T_3 &= \binom{n}{2} x^{n-2} y^2 = \frac{n(n-1)}{2} x^{n-2} y^2 = 720 \\
T_4 &= \binom{n}{3} x^{n-3} y^3 = \frac{n(n-1)(n-2)}{6} x^{n-3} y^3 = 1080
\end{align*}

Let's find ratios:
\[
\frac{T_3}{T_2} = \frac{\frac{n(n-1)}{2} x^{n-2} y^2}{n x^{n-1} y} = \frac{(n-1)y}{2x} = \frac{720}{240} = 3
\]

So $(n-1)y = 6x$.

\[
\frac{T_4}{T_3} = \frac{\frac{n(n-1)(n-2)}{6} x^{n-3} y^3}{\frac{n(n-1)}{2} x^{n-2} y^2} = \frac{(n-2)y}{3x} = \frac{1080}{720} = \frac{3}{2}
\]

So $(n-2)y = \frac{9x}{2}$.

From the two equations:
\begin{align*}
(n-1)y &= 6x \\
(n-2)y &= \frac{9x}{2}
\end{align*}

Dividing:
\[
\frac{(n-1)y}{(n-2)y} = \frac{6x}{\frac{9x}{2}} = \frac{6 \cdot 2}{9} = \frac{4}{3}
\]
\[
\frac{n-1}{n-2} = \frac{4}{3}
\]
\[
3(n-1) = 4(n-2)
\]
\[
3n - 3 = 4n - 8
\]
\[
n = 5
\]

From $(n-1)y = 6x$: $4y = 6x \Rightarrow y = \frac{3x}{2}$

Now use $T_2 = 240$:
\[
nx^{n-1}y = 5x^4 \cdot \frac{3x}{2} = \frac{15x^5}{2} = 240
\]
\[
x^5 = 32 \Rightarrow x = 2
\]

Then $y = \frac{3 \cdot 2}{2} = 3$.

Therefore: $x + y + n = 2 + 3 + 5 = 10$.

\subsection*{Answer}
\textbf{(C)} 10

\end{document}
