\documentclass[12pt]{article}
\usepackage[margin=1in]{geometry}
\usepackage{amsmath,amssymb}
\begin{document}

\section*{Problem 9}
If $f(x) = \left(\frac{x+1}{x-1}\right)^2$ for $x \neq \pm 1$, find $f\left(\frac{x+1}{x-1}\right) - f\left(\frac{x-1}{x+1}\right)$.

\subsection*{Solution}
First, let's compute $f\left(\frac{x+1}{x-1}\right)$.

Let $u = \frac{x+1}{x-1}$. Then:
\[
f(u) = \left(\frac{u+1}{u-1}\right)^2
\]

We need to find $\frac{u+1}{u-1}$ where $u = \frac{x+1}{x-1}$:
\[
u + 1 = \frac{x+1}{x-1} + 1 = \frac{x+1 + x-1}{x-1} = \frac{2x}{x-1}
\]
\[
u - 1 = \frac{x+1}{x-1} - 1 = \frac{x+1 - x+1}{x-1} = \frac{2}{x-1}
\]
\[
\frac{u+1}{u-1} = \frac{\frac{2x}{x-1}}{\frac{2}{x-1}} = \frac{2x}{2} = x
\]

So $f\left(\frac{x+1}{x-1}\right) = x^2$.

Now let's compute $f\left(\frac{x-1}{x+1}\right)$.

Let $v = \frac{x-1}{x+1}$. Then:
\[
v + 1 = \frac{x-1}{x+1} + 1 = \frac{x-1 + x+1}{x+1} = \frac{2x}{x+1}
\]
\[
v - 1 = \frac{x-1}{x+1} - 1 = \frac{x-1 - x-1}{x+1} = \frac{-2}{x+1}
\]
\[
\frac{v+1}{v-1} = \frac{\frac{2x}{x+1}}{\frac{-2}{x+1}} = \frac{2x}{-2} = -x
\]

So $f\left(\frac{x-1}{x+1}\right) = (-x)^2 = x^2$.

Therefore:
\[
f\left(\frac{x+1}{x-1}\right) - f\left(\frac{x-1}{x+1}\right) = x^2 - x^2 = 0
\]

\subsection*{Answer}
\textbf{(C)} 0

\end{document}
