\documentclass[12pt]{article}
\usepackage[margin=1in]{geometry}
\usepackage{amsmath,amssymb}
\begin{document}

\section*{Problem 2}
Find the value of the expression $\displaystyle\left(\frac{i^{2011} + i^{2012}}{i^{2013} - i^{2014}}\right)^{2015}$, where $i^2 = -1$.

\subsection*{Solution}
First, let's find the pattern of powers of $i$:
\begin{align*}
i^1 &= i \\
i^2 &= -1 \\
i^3 &= -i \\
i^4 &= 1
\end{align*}
The powers of $i$ cycle with period 4.

Now let's find each power modulo 4:
\begin{align*}
2011 &= 4 \cdot 502 + 3, \quad \text{so } i^{2011} = i^3 = -i \\
2012 &= 4 \cdot 503, \quad \text{so } i^{2012} = i^0 = 1 \\
2013 &= 4 \cdot 503 + 1, \quad \text{so } i^{2013} = i^1 = i \\
2014 &= 4 \cdot 503 + 2, \quad \text{so } i^{2014} = i^2 = -1
\end{align*}

Substituting:
\[
\frac{i^{2011} + i^{2012}}{i^{2013} - i^{2014}} = \frac{-i + 1}{i - (-1)} = \frac{1 - i}{1 + i}
\]

Multiply numerator and denominator by the conjugate of the denominator:
\[
\frac{1 - i}{1 + i} \cdot \frac{1 - i}{1 - i} = \frac{(1-i)^2}{1 - i^2} = \frac{1 - 2i + i^2}{1 - (-1)} = \frac{1 - 2i - 1}{2} = \frac{-2i}{2} = -i
\]

Therefore:
\[
\left(\frac{i^{2011} + i^{2012}}{i^{2013} - i^{2014}}\right)^{2015} = (-i)^{2015}
\]

Since $2015 = 4 \cdot 503 + 3$:
\[
(-i)^{2015} = ((-i)^4)^{503} \cdot (-i)^3 = 1^{503} \cdot (-i)^3 = (-1)^3 \cdot i^3 = -1 \cdot (-i) = i
\]

\subsection*{Answer}
\textbf{(D)} $i$

\end{document}
