\documentclass[12pt]{article}
\usepackage[margin=1in]{geometry}
\usepackage{amsmath,amssymb}
\begin{document}

\section*{Problem 8}
The limit $\lim_{x \to \infty} \left(\frac{x^3 - 6x^2 + 11x - 6}{x^2 - 6x + 9} - \frac{\sin(x - 3)}{\ln(2x - 5) + \cos \frac{\pi}{x}}\right)$ is:

\subsection*{Solution}
Let's analyze each part of the expression separately.

First, let's factor the polynomials:
- $x^3 - 6x^2 + 11x - 6 = (x-1)(x-2)(x-3)$
- $x^2 - 6x + 9 = (x-3)^2$

So the first fraction becomes:
\[
\frac{x^3 - 6x^2 + 11x - 6}{x^2 - 6x + 9} = \frac{(x-1)(x-2)(x-3)}{(x-3)^2} = \frac{(x-1)(x-2)}{x-3}
\]

As $x \to \infty$:
\[
\frac{(x-1)(x-2)}{x-3} = \frac{x^2 - 3x + 2}{x - 3} \sim \frac{x^2}{x} = x \to \infty
\]

More precisely:
\[
\frac{x^2 - 3x + 2}{x - 3} = x + \frac{2}{x-3} \to \infty
\]

For the second fraction, as $x \to \infty$:
- $\sin(x - 3)$ oscillates between -1 and 1
- $\ln(2x - 5) \to \infty$
- $\cos \frac{\pi}{x} \to \cos 0 = 1$

So $\ln(2x - 5) + \cos \frac{\pi}{x} \to \infty$, and therefore:
\[
\frac{\sin(x - 3)}{\ln(2x - 5) + \cos \frac{\pi}{x}} \to 0
\]

Therefore:
\[
\lim_{x \to \infty} \left(\frac{x^3 - 6x^2 + 11x - 6}{x^2 - 6x + 9} - \frac{\sin(x - 3)}{\ln(2x - 5) + \cos \frac{\pi}{x}}\right) = \infty - 0 = \infty
\]

Wait, let me double-check the polynomial factorization:
$x^3 - 6x^2 + 11x - 6$

Let me try $x = 1$: $1 - 6 + 11 - 6 = 0$ ✓
Let me try $x = 2$: $8 - 24 + 22 - 6 = 0$ ✓
Let me try $x = 3$: $27 - 54 + 33 - 6 = 0$ ✓

So indeed $x^3 - 6x^2 + 11x - 6 = (x-1)(x-2)(x-3)$.

The analysis above is correct, so the limit is $+\infty$.

\subsection*{Answer}
$+\infty$ (option \textbf{E}).

\end{document}