\documentclass[12pt]{article}
\usepackage[margin=1in]{geometry}
\usepackage{amsmath,amssymb}
\begin{document}

\section*{Problem 5}
If $\sin \alpha = -\frac{5}{13}$ and $\alpha \in \left(\frac{3\pi}{2}, 2\pi\right)$, then $\tan\left(\frac{\pi}{4} + \alpha\right)$ is:

\subsection*{Solution}
Given: $\sin \alpha = -\frac{5}{13}$ and $\alpha \in \left(\frac{3\pi}{2}, 2\pi\right)$ (fourth quadrant).

In the fourth quadrant, $\sin \alpha < 0$ and $\cos \alpha > 0$.

Using the Pythagorean identity: $\sin^2 \alpha + \cos^2 \alpha = 1$
\[
\left(-\frac{5}{13}\right)^2 + \cos^2 \alpha = 1
\]
\[
\frac{25}{169} + \cos^2 \alpha = 1
\]
\[
\cos^2 \alpha = 1 - \frac{25}{169} = \frac{169 - 25}{169} = \frac{144}{169}
\]

Since $\alpha$ is in the fourth quadrant, $\cos \alpha > 0$:
\[
\cos \alpha = \frac{12}{13}
\]

Therefore:
\[
\tan \alpha = \frac{\sin \alpha}{\cos \alpha} = \frac{-\frac{5}{13}}{\frac{12}{13}} = -\frac{5}{12}
\]

Now we use the tangent addition formula:
\[
\tan\left(\frac{\pi}{4} + \alpha\right) = \frac{\tan \frac{\pi}{4} + \tan \alpha}{1 - \tan \frac{\pi}{4} \tan \alpha}
\]

Since $\tan \frac{\pi}{4} = 1$:
\[
\tan\left(\frac{\pi}{4} + \alpha\right) = \frac{1 + \tan \alpha}{1 - \tan \alpha} = \frac{1 + \left(-\frac{5}{12}\right)}{1 - \left(-\frac{5}{12}\right)}
\]
\[
= \frac{1 - \frac{5}{12}}{1 + \frac{5}{12}} = \frac{\frac{12 - 5}{12}}{\frac{12 + 5}{12}} = \frac{\frac{7}{12}}{\frac{17}{12}} = \frac{7}{17}
\]

\subsection*{Answer}
$\frac{7}{17}$ (option \textbf{D}).

\end{document}