\documentclass[12pt]{article}
\usepackage[margin=1in]{geometry}
\usepackage{amsmath,amssymb}
\usepackage[utf8]{inputenc}
\begin{document}

\section*{Problem 8}
The limit $\lim_{x \to 2} \frac{\text{tg} \frac{3\pi x}{8} \cdot (\log(5x-9)+1) \cdot (\sqrt[3]{x} - \sqrt[3]{2})}{(x-2) \cdot (\sqrt{2x^3 - x - 5} - \sqrt{2x})}$ is equal to:

\subsection*{Solution}
We evaluate the limit of each factor as $x \to 2$.
1. $\text{tg} \frac{3\pi x}{8} \to \text{tg} \frac{3\pi (2)}{8} = \text{tg} \frac{3\pi}{4} = -1$.
2. $\log(5x-9)+1 \to \log(10-9)+1 = \log(1)+1 = 0+1 = 1$.
3. Denominator term $\sqrt{2x^3 - x - 5} - \sqrt{2x} \to \sqrt{16-2-5} - \sqrt{4} = \sqrt{9} - 2 = 3 - 2 = 1$.

So the limit simplifies to:
\[ (-1) \cdot (1) \cdot \lim_{x \to 2} \frac{\sqrt[3]{x} - \sqrt[3]{2}}{x-2} \cdot \frac{1}{1} \]
Let $L = \lim_{x \to 2} \frac{\sqrt[3]{x} - \sqrt[3]{2}}{x-2}$.
This is the derivative of $f(x) = x^{1/3}$ at $x=2$.
\[ f'(x) = \frac{1}{3}x^{-2/3} \]
\[ f'(2) = \frac{1}{3} (2)^{-2/3} = \frac{1}{3 \sqrt[3]{4}} = \frac{1}{3 \cdot 2^{2/3}} \]
Thus the total limit is:
\[ -1 \cdot \frac{1}{3 \cdot 2^{2/3}} = -\frac{1}{3 \cdot 2^{2/3}} \]

\subsection*{Answer}
$-\frac{1}{3 \cdot 2^{2/3}}$ (option \textbf{B}).

\end{document}
