\documentclass[12pt]{article}
\usepackage[margin=1in]{geometry}
\usepackage{amsmath,amssymb}
\usepackage[utf8]{inputenc}
\begin{document}

\section*{Problem 17}
The sum of all solutions to the equation
$(\sqrt{\log_7(-2x-1)} - \log_7 \sqrt{4x^2+4x+1} - 1) \cdot \log_7 |x+7| = -3 \log_7 \sqrt[3]{x+7}$
is:

\subsection*{Solution}
Domain constraints:
1. $\log_7(-2x-1)$ requires $-2x-1 > 0 \implies x < -1/2$.
2. Square root requires $\log_7(-2x-1) \ge 0 \implies -2x-1 \ge 1 \implies x \le -1$.
3. $\log_7 |x+7|$ requires $x \neq -7$.
4. $\log_7 \sqrt[3]{x+7}$ requires $x+7 > 0 \implies x > -7$.
Domain: $x \in (-7, -1]$.

Simplify the equation:
Note $\sqrt{4x^2+4x+1} = \sqrt{(2x+1)^2} = |2x+1|$.
Since $x \le -1$, $2x+1 < 0$, so $|2x+1| = -(2x+1) = -2x-1$.
Term $\log_7 \sqrt{4x^2+4x+1} = \log_7(-2x-1)$.
RHS: $-3 \log_7 (x+7)^{1/3} = -3 \cdot \frac{1}{3} \log_7(x+7) = -\log_7(x+7)$.

Equation becomes:
\[ (\sqrt{\log_7(-2x-1)} - \log_7(-2x-1) - 1) \log_7(x+7) = -\log_7(x+7) \]
\[ (\sqrt{\log_7(-2x-1)} - \log_7(-2x-1) - 1 + 1) \log_7(x+7) = 0 \]
\[ (\sqrt{\log_7(-2x-1)} - \log_7(-2x-1)) \log_7(x+7) = 0 \]

Case 1: $\log_7(x+7) = 0 \implies x+7 = 1 \implies x = -6$.
Valid since $-6 \in (-7, -1]$.

Case 2: $\sqrt{\log_7(-2x-1)} - \log_7(-2x-1) = 0$.
Let $t = \log_7(-2x-1)$.
$\sqrt{t} - t = 0 \implies \sqrt{t} = t \implies t = t^2 \implies t(t-1)=0$.
$t=0$ or $t=1$.
If $t=0$: $\log_7(-2x-1) = 0 \implies -2x-1 = 1 \implies x = -1$. Valid.
If $t=1$: $\log_7(-2x-1) = 1 \implies -2x-1 = 7 \implies x = -4$. Valid.

Solutions: $\{-6, -1, -4\}$.
Sum: $-6 - 1 - 4 = -11$.

\subsection*{Answer}
-11 (option \textbf{A}).

\end{document}
