\documentclass[12pt]{article}
\usepackage[margin=1in]{geometry}
\usepackage{amsmath,amssymb}
\usepackage[utf8]{inputenc}
\begin{document}

\section*{Problem 19}
The total number of real solutions to the system
$50\left(\frac{2}{5}\right)^{2x+3y-10} + 20\left(\frac{5}{2}\right)^{2x+3y-10} = 133$,
$(x+3)(y-1)=6$
is:

\subsection*{Solution}
Let $E = 2x+3y-10$ and $u = \left(\frac{2}{5}\right)^E$.
The first equation becomes:
\[ 50u + 20\frac{1}{u} = 133 \]
\[ 50u^2 - 133u + 20 = 0 \]
Solutions for $u$:
\[ u = \frac{133 \pm \sqrt{133^2 - 4000}}{100} = \frac{133 \pm 117}{100} \]
$u_1 = \frac{250}{100} = \frac{5}{2}$.
$u_2 = \frac{16}{100} = \frac{4}{25} = \left(\frac{2}{5}\right)^2$.

Case 1: $\left(\frac{2}{5}\right)^E = \frac{5}{2} = \left(\frac{2}{5}\right)^{-1} \implies E = -1$.
$2x + 3y - 10 = -1 \implies 2x = 9 - 3y$.
Substitute into $(x+3)(y-1)=6$:
$(\frac{9-3y}{2} + 3)(y-1) = 6$
$(15-3y)(y-1) = 12$
$3(5-y)(y-1) = 12 \implies (5-y)(y-1) = 4$
$-y^2 + 6y - 5 = 4 \implies y^2 - 6y + 9 = 0 \implies (y-3)^2 = 0$.
$y=3 \implies 2x = 9-9=0 \implies x=0$.
Solution $(0,3)$.

Case 2: $\left(\frac{2}{5}\right)^E = \left(\frac{2}{5}\right)^2 \implies E = 2$.
$2x + 3y - 10 = 2 \implies 2x = 12 - 3y$.
Substitute:
$(\frac{12-3y}{2} + 3)(y-1) = 6$
$(18-3y)(y-1) = 12$
$3(6-y)(y-1) = 12 \implies (6-y)(y-1) = 4$
$-y^2 + 7y - 6 = 4 \implies y^2 - 7y + 10 = 0$.
$(y-2)(y-5)=0$.
$y=2 \implies 2x = 6 \implies x=3$. Solution $(3,2)$.
$y=5 \implies 2x = -3 \implies x=-1.5$. Solution $(-1.5, 5)$.

Total solutions: 3.

\subsection*{Answer}
3 (option \textbf{D}).

\end{document}
