\documentclass[12pt]{article}
\usepackage[margin=1in]{geometry}
\usepackage{amsmath,amssymb}
\begin{document}

\section*{Problem 18}
The sum $1 + 11 + 111 + \cdots + \underbrace{11\ldots1}_{n}$ equals:

A) $\frac{1}{81}(10^{n+1} - 10 - 9n)$; B) $\frac{1}{9}(10^n - 9n + 8)$; C) $\frac{1}{81}(10^{n+1} - 19n)$; D) $\frac{1}{9}(10^{2n} - 40n - 50)$; E) $\frac{1}{11}(11^n - n + 1)$; N) Ne znam.

\subsection*{Solution}
Each term in the sum can be written as:
- $1 = \frac{10^1 - 1}{9}$
- $11 = \frac{10^2 - 1}{9}$  
- $111 = \frac{10^3 - 1}{9}$
- $\vdots$
- $\underbrace{11\ldots1}_{n} = \frac{10^n - 1}{9}$

So the sum is:
\[
S = \sum_{k=1}^{n} \frac{10^k - 1}{9} = \frac{1}{9}\sum_{k=1}^{n}(10^k - 1) = \frac{1}{9}\left(\sum_{k=1}^{n}10^k - \sum_{k=1}^{n}1\right)
\]

\[
= \frac{1}{9}\left(\sum_{k=1}^{n}10^k - n\right)
\]

The geometric series gives us:
\[
\sum_{k=1}^{n}10^k = 10 + 10^2 + \cdots + 10^n = 10\frac{10^n - 1}{10 - 1} = \frac{10(10^n - 1)}{9}
\]

Therefore:
\[
S = \frac{1}{9}\left(\frac{10(10^n - 1)}{9} - n\right) = \frac{1}{9} \cdot \frac{10(10^n - 1) - 9n}{9}
\]

\[
= \frac{10(10^n - 1) - 9n}{81} = \frac{10 \cdot 10^n - 10 - 9n}{81} = \frac{10^{n+1} - 10 - 9n}{81}
\]

\subsection*{Answer}
$\frac{1}{81}(10^{n+1} - 10 - 9n)$ (option \textbf{A}).

\end{document}