\documentclass[12pt]{article}
\usepackage[margin=1in]{geometry}
\usepackage{amsmath,amssymb}
\begin{document}

\section*{Problem 17}
The complex number $(1 + i\sqrt{3})^9 + (\sqrt{3} - i)^9$ $(i = \sqrt{-1})$ equals:

A) $2^9(1 + i)$; B) $2^9(-1 + i)$; C) $2^9(1 - i)$; D) $2^9$; E) $-2^9 i$; N) Ne znam.

\subsection*{Solution}
Let's convert to polar form.

For $z_1 = 1 + i\sqrt{3}$:
$|z_1| = \sqrt{1^2 + (\sqrt{3})^2} = \sqrt{1 + 3} = 2$
$\arg(z_1) = \arctan\left(\frac{\sqrt{3}}{1}\right) = \frac{\pi}{3}$

So $z_1 = 2\left(\cos\frac{\pi}{3} + i\sin\frac{\pi}{3}\right) = 2e^{i\pi/3}$

For $z_2 = \sqrt{3} - i$:
$|z_2| = \sqrt{(\sqrt{3})^2 + (-1)^2} = \sqrt{3 + 1} = 2$
$\arg(z_2) = \arctan\left(\frac{-1}{\sqrt{3}}\right) = -\frac{\pi}{6}$

So $z_2 = 2\left(\cos\left(-\frac{\pi}{6}\right) + i\sin\left(-\frac{\pi}{6}\right)\right) = 2e^{-i\pi/6}$

Using De Moivre's theorem:
\[
z_1^9 = 2^9 e^{i \cdot 9\pi/3} = 2^9 e^{3\pi i} = 2^9 e^{\pi i} = 2^9(-1) = -2^9
\]

\[
z_2^9 = 2^9 e^{-i \cdot 9\pi/6} = 2^9 e^{-3\pi i/2} = 2^9 e^{-3\pi i/2}
\]

Since $e^{-3\pi i/2} = e^{-3\pi i/2 + 2\pi i} = e^{\pi i/2} = i$:
\[
z_2^9 = 2^9 i
\]

Therefore:
\[
z_1^9 + z_2^9 = -2^9 + 2^9 i = 2^9(-1 + i)
\]

\subsection*{Answer}
$2^9(-1 + i)$ (option \textbf{B}).

\end{document}