\documentclass[12pt]{article}
\usepackage[margin=1in]{geometry}
\usepackage{amsmath,amssymb}
\usepackage[utf8]{inputenc}
\usepackage[T1]{fontenc}

\begin{document}

\section*{Problem 6}
Ako je $\frac{\cos(\alpha+\beta)}{\cos(\alpha-\beta)} = \frac{1}{3}$ ($\alpha, \beta \ne \frac{\pi}{2} + k\pi, \alpha-\beta \ne \frac{\pi}{2} + m\pi, k,m \in \mathbf{Z}$), tada je $\text{tg}\alpha \cdot \text{tg}\beta$ jednako:
\[ (A)\ \frac{1}{3} \quad (B)\ \frac{1}{2} \quad (C)\ 1 \quad (D)\ \frac{1}{4} \quad (E)\ \frac{2}{3} \quad (N)\ \text{Ne znam} \]

\subsection*{Solution}
Expand the cosine terms:
\[ \frac{\cos\alpha\cos\beta - \sin\alpha\sin\beta}{\cos\alpha\cos\beta + \sin\alpha\sin\beta} = \frac{1}{3} \]
Cross-multiply:
\[ 3(\cos\alpha\cos\beta - \sin\alpha\sin\beta) = \cos\alpha\cos\beta + \sin\alpha\sin\beta \]
\[ 3\cos\alpha\cos\beta - 3\sin\alpha\sin\beta = \cos\alpha\cos\beta + \sin\alpha\sin\beta \]
Group like terms:
\[ 3\cos\alpha\cos\beta - \cos\alpha\cos\beta = \sin\alpha\sin\beta + 3\sin\alpha\sin\beta \]
\[ 2\cos\alpha\cos\beta = 4\sin\alpha\sin\beta \]
Divide by $2\cos\alpha\cos\beta$ (assuming $\cos\alpha \ne 0, \cos\beta \ne 0$):
\[ 1 = 2 \frac{\sin\alpha\sin\beta}{\cos\alpha\cos\beta} \]
\[ 1 = 2 \text{tg}\alpha \text{tg}\beta \]
\[ \text{tg}\alpha \text{tg}\beta = \frac{1}{2} \]

\subsection*{Answer}
$\frac{1}{2}$ (option \textbf{B}).

\end{document}
