\documentclass[12pt]{article}
\usepackage[margin=1in]{geometry}
\usepackage{amsmath,amssymb}
\begin{document}

\section*{Problem 15}
Find the sum of all real solutions $x\in[0,2\pi]$ of
\[
\tan\!\left(x-\frac{\pi}{12}\right)\cdot \cot\!\left(x+\frac{\pi}{12}\right)=\frac{1}{3}.
\]

\subsection*{Solution}
Use $\cot\theta=\dfrac{1}{\tan\theta}$ (with $\tan\theta\neq 0$):
\[
\frac{\tan\!\left(x-\frac{\pi}{12}\right)}{\tan\!\left(x+\frac{\pi}{12}\right)}=\frac{1}{3}.
\]
Let $t=\tan\!\left(x+\frac{\pi}{12}\right)$. Then
\[
\tan\!\left(x-\frac{\pi}{12}\right)=\tan\!\left(\left(x+\frac{\pi}{12}\right)-\frac{\pi}{6}\right)
=\frac{t-\tan(\pi/6)}{1+t\tan(\pi/6)}
=\frac{t-\frac{1}{\sqrt3}}{1+\frac{t}{\sqrt3}}.
\]
The equation becomes
\[
\frac{t-\frac{1}{\sqrt3}}{1+\frac{t}{\sqrt3}}=\frac{t}{3}.
\]
Multiply out:
\[
t-\frac{1}{\sqrt3}=\frac{t}{3}\left(1+\frac{t}{\sqrt3}\right)=\frac{t}{3}+\frac{t^2}{3\sqrt3}.
\]
Multiply by $3\sqrt3$:
\[
3\sqrt3\,t-3=\sqrt3\,t+t^2
\quad\Longrightarrow\quad
t^2-2\sqrt3\,t+3=0.
\]
Discriminant is $12-12=0$, so $t=\sqrt3$.
Thus
\[
\tan\!\left(x+\frac{\pi}{12}\right)=\sqrt3
\quad\Longrightarrow\quad
x+\frac{\pi}{12}=\frac{\pi}{3}+k\pi
\]
\[
\Longrightarrow\quad x=\frac{\pi}{4}+k\pi.
\]
In $[0,2\pi]$ we get $x_1=\frac{\pi}{4}$ and $x_2=\frac{5\pi}{4}$. Their sum is
\[
\frac{\pi}{4}+\frac{5\pi}{4}=\frac{3\pi}{2}.
\]

\subsection*{Answer}
$\dfrac{3\pi}{2}$ (option \textbf{E}).

\end{document}

