\documentclass[12pt]{article}
\usepackage[margin=1in]{geometry}
\usepackage{amsmath,amssymb}
\begin{document}

\section*{Problem 8}
A sequence of functions $f_n : \mathbb{R} \to \mathbb{R}$ is defined with $f_1(x) = 2x + 2020$, $f_{n+1}(x) = f_1(f_n(x))$, $n \in \mathbb{N}$. Find $f_{2020}(-2020)$.

\subsection*{Solution}
First, let's find a pattern for $f_n(x)$.

$f_1(x) = 2x + 2020$

$f_2(x) = f_1(f_1(x)) = f_1(2x + 2020) = 2(2x + 2020) + 2020 = 4x + 4040 + 2020 = 4x + 6060$
$= 4x + 2020(2 + 1) = 4x + 2020 \cdot 3$

$f_3(x) = f_1(f_2(x)) = f_1(4x + 6060) = 2(4x + 6060) + 2020 = 8x + 12120 + 2020 = 8x + 14140$
$= 8x + 2020 \cdot 7$

Let's look for a pattern. It appears that:
\[
f_n(x) = 2^n x + 2020(2^n - 1)
\]

Let's verify by induction:
- Base case $n=1$: $f_1(x) = 2^1 x + 2020(2^1 - 1) = 2x + 2020$ âœ“
- Inductive step: Assume $f_n(x) = 2^n x + 2020(2^n - 1)$.
  
  Then:
  \[
  f_{n+1}(x) = f_1(f_n(x)) = 2(2^n x + 2020(2^n - 1)) + 2020
  \]
  \[
  = 2^{n+1} x + 2020 \cdot 2(2^n - 1) + 2020
  \]
  \[
  = 2^{n+1} x + 2020(2^{n+1} - 2 + 1)
  \]
  \[
  = 2^{n+1} x + 2020(2^{n+1} - 1) \checkmark
  \]

So the formula is confirmed: $f_n(x) = 2^n x + 2020(2^n - 1)$.

Now compute $f_{2020}(-2020)$:
\[
f_{2020}(-2020) = 2^{2020} \cdot (-2020) + 2020(2^{2020} - 1)
\]
\[
= -2020 \cdot 2^{2020} + 2020 \cdot 2^{2020} - 2020
\]
\[
= 2020(2^{2020} - 2^{2020}) - 2020
\]
\[
= -2020
\]

\subsection*{Answer}
$-2020$ (option \textbf{D}).

\end{document}
