\documentclass[12pt]{article}
\usepackage[margin=1in]{geometry}
\usepackage{amsmath,amssymb}
\begin{document}

\section*{Problem 4}
The inverse function of $f : [3, +\infty) \to [3, +\infty)$ with $f(x) = 3\sqrt{x-3} + 3$ is the function $g : [3, +\infty) \to [3, +\infty)$. Find $g(x)$.

\subsection*{Solution}
To find the inverse function, we set $y = f(x)$ and solve for $x$ in terms of $y$.

\[
y = 3\sqrt{x-3} + 3
\]

Subtract 3 from both sides:
\[
y - 3 = 3\sqrt{x-3}
\]

Divide by 3:
\[
\frac{y-3}{3} = \sqrt{x-3}
\]

Square both sides:
\[
\left(\frac{y-3}{3}\right)^2 = x - 3
\]

\[
\frac{(y-3)^2}{9} = x - 3
\]

Add 3 to both sides:
\[
x = \frac{(y-3)^2}{9} + 3
\]

Expanding $(y-3)^2 = y^2 - 6y + 9$:
\[
x = \frac{y^2 - 6y + 9}{9} + 3 = \frac{1}{9}y^2 - \frac{6}{9}y + \frac{9}{9} + 3
\]
\[
x = \frac{1}{9}y^2 - \frac{2}{3}y + 1 + 3 = \frac{1}{9}y^2 - \frac{2}{3}y + 4
\]

Therefore, the inverse function is:
\[
g(x) = \frac{1}{9}x^2 - \frac{2}{3}x + 4
\]

\subsection*{Answer}
$g(x) = \frac{1}{9}x^2 - \frac{2}{3}x + 4$ (option \textbf{A}).

\end{document}
