\documentclass[12pt]{article}
\usepackage[margin=1in]{geometry}
\usepackage{amsmath,amssymb}
\begin{document}

\section*{Problem 7}
Find the real part of the complex number $(z - z^2 + 2z^3)(2 - z + z^2)$, where $z = \frac{-1 + i\sqrt{3}}{2}$, $i^2 = -1$.

\subsection*{Solution}
First, let's recognize that $z = \frac{-1 + i\sqrt{3}}{2}$ is a primitive cube root of unity, often denoted $\omega$.

We know that $\omega^3 = 1$ and $1 + \omega + \omega^2 = 0$.

Let's verify: $z = e^{i \cdot 2\pi/3} = \cos(120°) + i\sin(120°) = -\frac{1}{2} + i\frac{\sqrt{3}}{2}$ ✓

Properties of $\omega$:
\begin{itemize}
    \item $\omega^3 = 1$
    \item $\omega^2 = \frac{-1 - i\sqrt{3}}{2}$
    \item $1 + \omega + \omega^2 = 0$
\end{itemize}

Now let's compute the expression $(z - z^2 + 2z^3)(2 - z + z^2)$.

Since $z^3 = 1$:
\[
z - z^2 + 2z^3 = z - z^2 + 2
\]

For the second factor:
\[
2 - z + z^2
\]

Now multiply:
\[
(z - z^2 + 2)(2 - z + z^2)
\]

Let's expand:
\[
= z(2 - z + z^2) - z^2(2 - z + z^2) + 2(2 - z + z^2)
\]
\[
= 2z - z^2 + z^3 - 2z^2 + z^3 - z^4 + 4 - 2z + 2z^2
\]

Using $z^3 = 1$ and $z^4 = z$:
\[
= 2z - z^2 + 1 - 2z^2 + 1 - z + 4 - 2z + 2z^2
\]
\[
= (2z - z - 2z) + (-z^2 - 2z^2 + 2z^2) + (1 + 1 + 4)
\]
\[
= -z - z^2 + 6
\]

Since $1 + z + z^2 = 0$, we have $z + z^2 = -1$.

Therefore:
\[
-z - z^2 + 6 = -(z + z^2) + 6 = -(-1) + 6 = 1 + 6 = 7
\]

Wait, but we need the real part. Since the result is $7$, which is a real number, the real part is $7$.

But let me double-check option (C) says 4. Let me recalculate...

Actually, let me recalculate more carefully:
\[
(z - z^2 + 2z^3)(2 - z + z^2)
\]

With $z^3 = 1$:
\[
= (z - z^2 + 2)(2 - z + z^2)
\]

Expanding term by term:
- $z \cdot 2 = 2z$
- $z \cdot (-z) = -z^2$
- $z \cdot z^2 = z^3 = 1$
- $(-z^2) \cdot 2 = -2z^2$
- $(-z^2) \cdot (-z) = z^3 = 1$
- $(-z^2) \cdot z^2 = -z^4 = -z$
- $2 \cdot 2 = 4$
- $2 \cdot (-z) = -2z$
- $2 \cdot z^2 = 2z^2$

Sum: $2z - z^2 + 1 - 2z^2 + 1 - z + 4 - 2z + 2z^2$

Collecting terms:
- $z$ terms: $2z - z - 2z = -z$
- $z^2$ terms: $-z^2 - 2z^2 + 2z^2 = -z^2$
- Constants: $1 + 1 + 4 = 6$

Result: $-z - z^2 + 6 = -(z + z^2) + 6 = -(-1) + 6 = 7$

Hmm, I get 7, but let me check if perhaps the question asks for something different or I misread.

Actually wait - looking at option (C) = 4, let me reconsider. Maybe I should compute directly.

$z = \frac{-1 + i\sqrt{3}}{2}$

$z^2 = \frac{1 - 2i\sqrt{3} - 3}{4} = \frac{-2 - 2i\sqrt{3}}{4} = \frac{-1 - i\sqrt{3}}{2}$

$z + z^2 = \frac{-1 + i\sqrt{3}}{2} + \frac{-1 - i\sqrt{3}}{2} = \frac{-2}{2} = -1$ ✓

So the result is indeed $7 - 0i$, and the real part is $7$.

But wait, looking at the options again: (A) $4(1 + \text{Im}^2 z)$, (B) $0$, (C) $4$, (D) $-\frac{1}{2}$, (E) $-\text{Re}z + 1$.

$\text{Im}(z) = \frac{\sqrt{3}}{2}$, so $\text{Im}^2(z) = \frac{3}{4}$.

Option (A): $4(1 + \frac{3}{4}) = 4 \cdot \frac{7}{4} = 7$ ✓

\subsection*{Answer}
$4(1 + \text{Im}^2 z) = 7$ (option \textbf{A}).

\end{document}
