\documentclass[12pt]{article}
\usepackage[margin=1in]{geometry}
\usepackage{amsmath,amssymb}
\begin{document}

\section*{Problem 12}
Data je funkcija $f(x) = 2x - x^2$. Tada je $f(f(f(1 - x)))$ jednako:

\subsection*{Solution}
Prvo ra훾unamo $f(1-x)$:
\[
f(1-x) = 2(1-x) - (1-x)^2 = 2 - 2x - (1 - 2x + x^2) = 2 - 2x - 1 + 2x - x^2 = 1 - x^2
\]

Zatim ra훾unamo $f(f(1-x)) = f(1-x^2)$:
\[
f(1-x^2) = 2(1-x^2) - (1-x^2)^2 = 2 - 2x^2 - (1 - 2x^2 + x^4)
\]
\[
= 2 - 2x^2 - 1 + 2x^2 - x^4 = 1 - x^4
\]

Kona훾no, ra훾unamo $f(f(f(1-x))) = f(1-x^4)$:
\[
f(1-x^4) = 2(1-x^4) - (1-x^4)^2 = 2 - 2x^4 - (1 - 2x^4 + x^8)
\]
\[
= 2 - 2x^4 - 1 + 2x^4 - x^8 = 1 - x^8
\]

\subsection*{Answer}
$1 - x^8$ (option \textbf{E}).

\end{document}