\documentclass[12pt]{article}
\usepackage[margin=1in]{geometry}
\usepackage{amsmath,amssymb}
\begin{document}

\section*{Problem 6}
Given the function $f(x) = x - \sin\pi x \cdot \cos\pi x + \frac{\ln 2x}{x} + e^{\text{tg}2\pi x}$. Find the value of $f'\left(\frac{1}{2}\right)$.

(A) $0$ \quad (B) $5 + 3\pi$ \quad (C) $3\pi$ \quad (D) $5$ \quad (E) $e$

\subsection*{Solution}
Let's compute the derivative of each term.

First, note that $\sin\pi x \cdot \cos\pi x = \frac{1}{2}\sin 2\pi x$, so:
\[
f(x) = x - \frac{1}{2}\sin 2\pi x + \frac{\ln 2x}{x} + e^{\tan 2\pi x}
\]

Taking the derivative:
\[
f'(x) = 1 - \frac{1}{2} \cdot 2\pi \cos 2\pi x + \frac{d}{dx}\left(\frac{\ln 2x}{x}\right) + e^{\tan 2\pi x} \cdot \frac{2\pi}{\cos^2 2\pi x}
\]

For $\frac{\ln 2x}{x}$, using the quotient rule:
\[
\frac{d}{dx}\left(\frac{\ln 2x}{x}\right) = \frac{\frac{1}{x} \cdot x - \ln 2x \cdot 1}{x^2} = \frac{1 - \ln 2x}{x^2}
\]

So:
\[
f'(x) = 1 - \pi\cos 2\pi x + \frac{1 - \ln 2x}{x^2} + \frac{2\pi e^{\tan 2\pi x}}{\cos^2 2\pi x}
\]

At $x = \frac{1}{2}$:
\begin{itemize}
\item $2\pi \cdot \frac{1}{2} = \pi$
\item $\cos \pi = -1$
\item $\tan \pi = 0$
\item $\cos^2 \pi = 1$
\item $\ln(2 \cdot \frac{1}{2}) = \ln 1 = 0$
\end{itemize}

\[
f'\left(\frac{1}{2}\right) = 1 - \pi(-1) + \frac{1 - 0}{(1/2)^2} + \frac{2\pi e^0}{1}
\]
\[
= 1 + \pi + \frac{1}{1/4} + 2\pi = 1 + \pi + 4 + 2\pi = 5 + 3\pi
\]

\subsection*{Answer}
(B) $5 + 3\pi$

\end{document}
