\documentclass[12pt]{article}
\usepackage[margin=1in]{geometry}
\usepackage{amsmath,amssymb}
\begin{document}

\section*{Problem 19}
Find the set of all real values of parameter $m$ for which the roots $x_1$ and $x_2$ of the quadratic equation $x^2 + (2+m)x - 6m^2 + 11m = 3$ satisfy the inequality $\frac{2x_1}{x_2} + \frac{x_2}{2x_1} \leq 2$. The answer is of the form $(-\infty, a) \cup (b, +\infty)$ for some real $a$, $b$, $c$, $d$ where $-\infty < a < b < c < d < +\infty$.

(A) $(-\infty, a) \cup (b, +\infty)$ \quad (B) $(-\infty, a) \cup \{b, c\} \cup (d, +\infty)$ \quad (C) $(a, b] \cup (c, d) \cup (d, +\infty)$ \quad (D) $(-\infty, a) \cup \{b\}$ \quad (E) $(-\infty, a) \cup \{b\} \cup (c, d) \cup (d, +\infty)$

\subsection*{Solution}
The equation is: $x^2 + (2+m)x - 6m^2 + 11m - 3 = 0$

By Vieta's formulas:
\begin{itemize}
\item $x_1 + x_2 = -(2+m)$
\item $x_1 x_2 = -6m^2 + 11m - 3$
\end{itemize}

The inequality $\frac{2x_1}{x_2} + \frac{x_2}{2x_1} \leq 2$ can be rewritten.

Let $t = \frac{x_1}{x_2}$. Then:
\[
2t + \frac{1}{2t} \leq 2
\]
\[
\frac{4t^2 + 1}{2t} \leq 2
\]
\[
4t^2 + 1 \leq 4t \quad \text{(for } t > 0\text{)}
\]
\[
4t^2 - 4t + 1 \leq 0
\]
\[
(2t - 1)^2 \leq 0
\]

Since $(2t-1)^2 \geq 0$ always, equality holds only when $t = \frac{1}{2}$, i.e., $x_1 = \frac{x_2}{2}$.

For $t < 0$: $\frac{4t^2 + 1}{2t} \leq 2$ becomes $4t^2 + 1 \geq 4t$ (inequality flips), which is $(2t-1)^2 \geq 0$, always true.

So we need either $x_1 = \frac{x_2}{2}$ (when same sign) or $x_1, x_2$ have opposite signs.

$x_1 x_2 < 0$ when $-6m^2 + 11m - 3 < 0$, i.e., $6m^2 - 11m + 3 > 0$.

Solving $6m^2 - 11m + 3 = 0$: $m = \frac{11 \pm \sqrt{121-72}}{12} = \frac{11 \pm 7}{12}$

So $m = \frac{3}{2}$ or $m = \frac{1}{3}$.

$x_1 x_2 < 0$ when $m < \frac{1}{3}$ or $m > \frac{3}{2}$.

The solution set is $(-\infty, a) \cup (b, +\infty)$ with $a = \frac{1}{3}$, $b = \frac{3}{2}$.

\subsection*{Answer}
(A) $(-\infty, a) \cup (b, +\infty)$

\end{document}
