\documentclass[12pt]{article}
\usepackage[margin=1in]{geometry}
\usepackage{amsmath,amssymb}
\begin{document}

\section*{Problem 7}
Find the limit:
\[
\lim_{x \to 5\pi} \frac{\left(e^{-\frac{1}{(5\pi-x)^2}+\sqrt{3\pi}}\right) \cdot \log_2 \frac{x+3\pi}{2\pi}}{\left(\sqrt{6x-5\pi}-2\sqrt{\pi}\right) \cdot \tan\left(\frac{x}{5}-\frac{4\pi}{3}\right)}
\]

(A) $\frac{\pi}{3}$ \quad (B) $0$ \quad (C) $+\infty$ \quad (D) $-\infty$ \quad (E) $-\frac{2}{3}$

\subsection*{Solution}
As $x \to 5\pi$:

\textbf{Numerator analysis:}
\begin{itemize}
\item As $x \to 5\pi$, $(5\pi - x)^2 \to 0^+$, so $-\frac{1}{(5\pi-x)^2} \to -\infty$
\item Therefore $e^{-\frac{1}{(5\pi-x)^2}+\sqrt{3\pi}} \to e^{-\infty} = 0$
\item $\log_2 \frac{5\pi + 3\pi}{2\pi} = \log_2 4 = 2$ (finite)
\end{itemize}

So the numerator $\to 0 \cdot 2 = 0$.

\textbf{Denominator analysis:}
\begin{itemize}
\item $\sqrt{6 \cdot 5\pi - 5\pi} - 2\sqrt{\pi} = \sqrt{25\pi} - 2\sqrt{\pi} = 5\sqrt{\pi} - 2\sqrt{\pi} = 3\sqrt{\pi}$
\item $\tan\left(\frac{5\pi}{5} - \frac{4\pi}{3}\right) = \tan\left(\pi - \frac{4\pi}{3}\right) = \tan\left(-\frac{\pi}{3}\right) = -\sqrt{3}$
\end{itemize}

So the denominator $\to 3\sqrt{\pi} \cdot (-\sqrt{3}) = -3\sqrt{3\pi}$ (finite, non-zero).

Since numerator $\to 0$ and denominator $\to$ finite non-zero:
\[
\lim_{x \to 5\pi} = \frac{0}{-3\sqrt{3\pi}} = 0
\]

\subsection*{Answer}
(B) $0$

\end{document}
