\documentclass[12pt]{article}
\usepackage[margin=1in]{geometry}
\usepackage{amsmath,amssymb}
\begin{document}

\section*{Problem 9}
Ako je
\[
f(x)=\frac{4}{x-5}+(3x+1)e^{-(x-1)^2}+\sqrt{-2x+3},
\]
odrediti $f'(1)$.

\subsection*{Solution}
Derivišemo član po član.

\medskip
\textbf{1) } $\displaystyle \frac{4}{x-5}=4(x-5)^{-1}\Rightarrow \left(\frac{4}{x-5}\right)'=-4(x-5)^{-2}$, pa
\[
\left(\frac{4}{x-5}\right)'\Big|_{x=1}=-\frac{4}{(1-5)^2}=-\frac{4}{16}=-\frac14.
\]

\medskip
\textbf{2) } $g(x)=(3x+1)e^{-(x-1)^2}$.
Primena pravila proizvoda daje
\[
g'(x)=3e^{-(x-1)^2}+(3x+1)e^{-(x-1)^2}\cdot\big(-2(x-1)\big).
\]
Za $x=1$ je $e^{0}=1$ i drugi sabirak nestaje, pa je $g'(1)=3$.

\medskip
\textbf{3) } $h(x)=\sqrt{-2x+3}=(-2x+3)^{1/2}$, pa
\[
h'(x)=\frac12(-2x+3)^{-1/2}\cdot(-2)=-( -2x+3)^{-1/2},
\]
odakle je $h'(1)=-1$.

\medskip
Zato je
\[
f'(1)=-\frac14+3-1=\frac74.
\]

\subsection*{Answer}
$\dfrac74$ (option \textbf{E}).

\end{document}

