\documentclass[12pt]{article}
\usepackage[margin=1in]{geometry}
\usepackage{amsmath,amssymb}
\begin{document}

\section*{Problem 8}
Skup svih rešenja nejednačine $\displaystyle\frac{(x+1)(x+2)}{(x-1)(x-2)} \geq 1$ je:

(A) $(-\infty, +\infty)$ \quad (B) $[0, +\infty)$ \quad (C) $[0, 1]$ \quad (D) $[0, 1) \cup (2, +\infty)$ \quad (E) $(-\infty, 0] \cup (2, +\infty)$ \quad (N) Ne znam

\subsection*{Solution}
We solve $\displaystyle\frac{(x+1)(x+2)}{(x-1)(x-2)} \geq 1$.

Rearranging:
\[
\frac{(x+1)(x+2)}{(x-1)(x-2)} - 1 \geq 0
\]
\[
\frac{(x+1)(x+2) - (x-1)(x-2)}{(x-1)(x-2)} \geq 0
\]

Expanding the numerator:
\begin{align*}
(x+1)(x+2) &= x^2 + 3x + 2 \\
(x-1)(x-2) &= x^2 - 3x + 2 \\
(x+1)(x+2) - (x-1)(x-2) &= (x^2 + 3x + 2) - (x^2 - 3x + 2) = 6x
\end{align*}

So we need:
\[
\frac{6x}{(x-1)(x-2)} \geq 0
\]

The critical points are $x = 0$, $x = 1$, $x = 2$.

Sign analysis:
\begin{itemize}
\item For $x < 0$: $6x < 0$, $(x-1) < 0$, $(x-2) < 0$ $\Rightarrow$ $\frac{(-)}{(-)(-))} = \frac{(-)}{(+)} < 0$
\item For $0 < x < 1$: $6x > 0$, $(x-1) < 0$, $(x-2) < 0$ $\Rightarrow$ $\frac{(+)}{(-)(-))} = \frac{(+)}{(+)} > 0$
\item For $1 < x < 2$: $6x > 0$, $(x-1) > 0$, $(x-2) < 0$ $\Rightarrow$ $\frac{(+)}{(+)(-))} = \frac{(+)}{(-)} < 0$
\item For $x > 2$: $6x > 0$, $(x-1) > 0$, $(x-2) > 0$ $\Rightarrow$ $\frac{(+)}{(+)(+))} = \frac{(+)}{(+)} > 0$
\end{itemize}

At $x = 0$: the expression equals $0$, so it satisfies $\geq 0$.

At $x = 1$ and $x = 2$: the expression is undefined.

Solution set: $\{0\} \cup (0, 1) \cup (2, +\infty) = [0, 1) \cup (2, +\infty)$

\subsection*{Answer}
$[0, 1) \cup (2, +\infty)$ (option \textbf{D}).

\end{document}
