\documentclass[12pt]{article}
\usepackage[margin=1in]{geometry}
\usepackage{amsmath,amssymb}
\begin{document}

\section*{Problem 4}
Vrednost izraza $\displaystyle\frac{(1+i)^{2008} - (1-i)^{2009}}{(1+i)^{2006} + (1-i)^{2007}}$, $(i^2 = -1)$ iznosi:

(A) $i$ \quad (B) $1+i$ \quad (C) $1-i$ \quad (D) $-i$ \quad (E) $2i$ \quad (N) Ne znam

\subsection*{Solution}
First, let's find the polar forms:
\[
1 + i = \sqrt{2} \cdot e^{i\pi/4}, \quad 1 - i = \sqrt{2} \cdot e^{-i\pi/4}
\]

Powers of $1+i$ and $1-i$:
\[
(1+i)^2 = 1 + 2i - 1 = 2i, \quad (1-i)^2 = 1 - 2i - 1 = -2i
\]

So $(1+i)^4 = (2i)^2 = -4$ and $(1-i)^4 = (-2i)^2 = -4$.

Since $2008 = 4 \cdot 502$, we have $(1+i)^{2008} = (-4)^{502} = 4^{502}$.

Since $2006 = 4 \cdot 501 + 2$, we have $(1+i)^{2006} = (-4)^{501} \cdot 2i = -4^{501} \cdot 2i$.

Since $2009 = 4 \cdot 502 + 1$, we have $(1-i)^{2009} = (-4)^{502} \cdot (1-i) = 4^{502}(1-i)$.

Since $2007 = 4 \cdot 501 + 3$, we have $(1-i)^{2007} = (-4)^{501} \cdot (1-i)^3$.

Now $(1-i)^3 = (1-i)^2 \cdot (1-i) = -2i(1-i) = -2i + 2i^2 = -2 - 2i$.

So $(1-i)^{2007} = -4^{501}(-2-2i) = 4^{501}(2+2i)$.

Numerator:
\[
(1+i)^{2008} - (1-i)^{2009} = 4^{502} - 4^{502}(1-i) = 4^{502}(1 - 1 + i) = 4^{502} \cdot i
\]

Denominator:
\[
(1+i)^{2006} + (1-i)^{2007} = -4^{501} \cdot 2i + 4^{501}(2+2i) = 4^{501}(-2i + 2 + 2i) = 4^{501} \cdot 2
\]

Therefore:
\[
\frac{4^{502} \cdot i}{4^{501} \cdot 2} = \frac{4 \cdot i}{2} = 2i
\]

\subsection*{Answer}
$2i$ (option \textbf{E}).

\end{document}
