\documentclass[12pt]{article}
\usepackage[margin=1in]{geometry}
\usepackage{amsmath,amssymb}
\begin{document}

\section*{Problem 1}
Vrednost izraza $2^{0.5} - 2^0 - (2^{0.5} + 2^0)^{-1}$ jednaka je:

(A) 0 \quad (B) 1 \quad (C) 2 \quad (D) $\sqrt{2}$ \quad (E) $-\sqrt{2}$ \quad (N) Ne znam

\subsection*{Solution}
Let us compute step by step:
\begin{align*}
2^{0.5} &= \sqrt{2} \\
2^0 &= 1 \\
2^{0.5} + 2^0 &= \sqrt{2} + 1 \\
(2^{0.5} + 2^0)^{-1} &= \frac{1}{\sqrt{2} + 1}
\end{align*}

To simplify $\frac{1}{\sqrt{2} + 1}$, we rationalize the denominator:
\[
\frac{1}{\sqrt{2} + 1} \cdot \frac{\sqrt{2} - 1}{\sqrt{2} - 1} = \frac{\sqrt{2} - 1}{2 - 1} = \sqrt{2} - 1
\]

Now we compute the full expression:
\[
2^{0.5} - 2^0 - (2^{0.5} + 2^0)^{-1} = \sqrt{2} - 1 - (\sqrt{2} - 1) = \sqrt{2} - 1 - \sqrt{2} + 1 = 0
\]

\subsection*{Answer}
$0$ (option \textbf{A}).

\end{document}
