\documentclass[12pt]{article}
\usepackage[margin=1in]{geometry}
\usepackage{amsmath,amssymb}
\begin{document}

\section*{Problem 11}
Let $x \in \mathbb{R}$ be a positive number and let $n \in \mathbb{N}$ be an even number. The sum of all binomial coefficients in the expansion of $\left(x^{2019} + \frac{1}{x^{2019}}\right)^n$ is four times greater than the sum of all binomial coefficients in the expansion of $\left(\sqrt{x} + \frac{1}{\sqrt{x}}\right)^{\frac{n}{2}}$. The sum of those members of the two expansions that do not contain $x$ is:

\subsection*{Solution}
The sum of all binomial coefficients in $(a + b)^k$ is $2^k$ (obtained by setting $a = b = 1$).

For the first expansion $\left(x^{2019} + \frac{1}{x^{2019}}\right)^n$:
Sum of binomial coefficients = $2^n$

For the second expansion $\left(\sqrt{x} + \frac{1}{\sqrt{x}}\right)^{\frac{n}{2}}$:
Sum of binomial coefficients = $2^{n/2}$

Given condition: $2^n = 4 \cdot 2^{n/2}$
$2^n = 2^2 \cdot 2^{n/2} = 2^{2 + n/2}$

This gives us: $n = 2 + \frac{n}{2}$
$n - \frac{n}{2} = 2$
$\frac{n}{2} = 2$
$n = 4$

Now we need to find the terms that don't contain $x$ in both expansions.

\textbf{First expansion:} $\left(x^{2019} + \frac{1}{x^{2019}}\right)^4$

The general term is: $\binom{4}{k}(x^{2019})^k\left(\frac{1}{x^{2019}}\right)^{4-k} = \binom{4}{k}x^{2019k}x^{-2019(4-k)} = \binom{4}{k}x^{2019(2k-4)}$

For the term to not contain $x$, we need: $2019(2k-4) = 0$
Since $2019 \neq 0$, we need $2k - 4 = 0$, so $k = 2$.

The constant term is: $\binom{4}{2} = 6$

\textbf{Second expansion:} $\left(\sqrt{x} + \frac{1}{\sqrt{x}}\right)^2$

The general term is: $\binom{2}{j}(\sqrt{x})^j\left(\frac{1}{\sqrt{x}}\right)^{2-j} = \binom{2}{j}x^{j/2}x^{-(2-j)/2} = \binom{2}{j}x^{(j-2+j)/2} = \binom{2}{j}x^{j-1}$

For the term to not contain $x$, we need: $j - 1 = 0$, so $j = 1$.

The constant term is: $\binom{2}{1} = 2$

Therefore, the sum of terms that don't contain $x$ is: $6 + 2 = 8$

\subsection*{Answer}
8 (option \textbf{C}).

\end{document}