\documentclass[12pt]{article}
\usepackage[margin=1in]{geometry}
\usepackage{amsmath,amssymb}
\begin{document}

\section*{Problem 8}
The limit $\lim_{x \to \infty} \left(\frac{x^3 - 6x^2 + 11x - 6}{x^2 - 6x + 9} - \frac{\sin(x-3)}{\ln(2x-5) + \cos\frac{\pi}{x}}\right)$ equals:

\subsection*{Solution}
Let's analyze each part of the expression separately.

\textbf{First part:} $\frac{x^3 - 6x^2 + 11x - 6}{x^2 - 6x + 9}$

Let's factor the polynomials:
- $x^3 - 6x^2 + 11x - 6 = (x-1)(x-2)(x-3)$
- $x^2 - 6x + 9 = (x-3)^2$

So: $\frac{x^3 - 6x^2 + 11x - 6}{x^2 - 6x + 9} = \frac{(x-1)(x-2)(x-3)}{(x-3)^2} = \frac{(x-1)(x-2)}{x-3}$

As $x \to \infty$:
$\frac{(x-1)(x-2)}{x-3} = \frac{x^2 - 3x + 2}{x - 3} \approx \frac{x^2}{x} = x \to \infty$

More precisely, using polynomial long division:
$\frac{x^2 - 3x + 2}{x - 3} = x + \frac{2}{x-3}$

As $x \to \infty$: $x + \frac{2}{x-3} \to \infty$

\textbf{Second part:} $\frac{\sin(x-3)}{\ln(2x-5) + \cos\frac{\pi}{x}}$

As $x \to \infty$:
- $\sin(x-3)$ oscillates between -1 and 1
- $\ln(2x-5) \to \infty$
- $\cos\frac{\pi}{x} \to \cos(0) = 1$

So the denominator $\ln(2x-5) + \cos\frac{\pi}{x} \to \infty + 1 = \infty$

Therefore: $\frac{\sin(x-3)}{\ln(2x-5) + \cos\frac{\pi}{x}} \to 0$

\textbf{Combining both parts:}
The limit becomes:
$\lim_{x \to \infty} \left(\frac{(x-1)(x-2)}{x-3} - \frac{\sin(x-3)}{\ln(2x-5) + \cos\frac{\pi}{x}}\right)$

Since the first part goes to infinity and the second part goes to 0, the limit is $+\infty$.

However, let me reconsider the first part more carefully:
$\frac{x^2 - 3x + 2}{x - 3} = x + \frac{2}{x-3}$

As $x \to \infty$, this approaches $x$, which goes to infinity.

But looking at the answer choices, let me check if there's a different interpretation or if I made an error.

Actually, let me be more careful with the polynomial division:
$\frac{x^2 - 3x + 2}{x - 3} = x + 0 + \frac{2}{x-3} = x + \frac{2}{x-3}$

As $x \to \infty$, this is indeed $\infty$.

Given the answer choices include finite values, let me double-check my factorization:
$x^3 - 6x^2 + 11x - 6$

Let me verify: $(x-1)(x-2)(x-3) = (x-1)(x^2 - 5x + 6) = x^3 - 5x^2 + 6x - x^2 + 5x - 6 = x^3 - 6x^2 + 11x - 6$ ✓

And $x^2 - 6x + 9 = (x-3)^2$ ✓

So the simplification is correct: $\frac{(x-1)(x-2)}{x-3}$

Since this goes to infinity, and the second term goes to 0, the overall limit should be $+\infty$.

Looking at the options, (E) is $+\infty$, which matches our calculation.

\subsection*{Answer}
$+\infty$ (option \textbf{E}).

\end{document}