\documentclass[12pt]{article}
\usepackage[margin=1in]{geometry}
\usepackage{amsmath,amssymb}
\begin{document}

\section*{Problem 3}
Izra\v{c}unati vrednost izraza
\[
\left(\frac{x-9}{x+3\sqrt{x}+9}:\frac{x^{0.5}+3}{x^{1.5}-27}\right)^{0.5}-x^{0.5},
\qquad x\in(9,+\infty).
\]

\subsection*{Solution}
Neka je $t=\sqrt{x}$, pa je $t>3$ i $x=t^2$.
Tada va\v{z}i
\[
\frac{x-9}{x+3\sqrt{x}+9}=\frac{t^2-9}{t^2+3t+9}=\frac{(t-3)(t+3)}{t^2+3t+9},
\]
kao i
\[
\frac{x^{0.5}+3}{x^{1.5}-27}=\frac{t+3}{t^3-27}
=\frac{t+3}{(t-3)(t^2+3t+9)}.
\]
Zato je koli\v{c}nik u zagradi
\begin{align*}
\frac{\frac{x-9}{x+3\sqrt{x}+9}}{\frac{x^{0.5}+3}{x^{1.5}-27}}
&=
\frac{(t-3)(t+3)}{t^2+3t+9}\cdot
\frac{(t-3)(t^2+3t+9)}{t+3}
=(t-3)^2.
\end{align*}
Sledi
\[
\left((t-3)^2\right)^{0.5} = |t-3| = t-3 \quad (t>3).
\]
Zato je ceo izraz jednak
\[
(t-3)-t=-3.
\]

\subsection*{Answer}
$-3$ (option \textbf{C}).

\end{document}

