\documentclass[12pt]{article}
\usepackage[margin=1in]{geometry}
\usepackage{amsmath,amssymb}
\begin{document}

\section*{Problem 19}
Ako je $\cos x : \cos 2x : \cos 4x = 1 : 2 : y$, tada je $y$ jednako:

\textbf{A)} 4; \quad \textbf{B)} $5 + 3\sqrt{3}$; \quad \textbf{C)} 8; \quad \textbf{D)} $5 - 3\sqrt{3}$; \quad \textbf{E)} $4 - 3\sqrt{3}$

\subsection*{Solution}
Iz proporcije $\cos x : \cos 2x = 1 : 2$ sledi:
\[
\frac{\cos x}{\cos 2x} = \frac{1}{2}
\]
\[
2\cos x = \cos 2x
\]

Koristimo $\cos 2x = 2\cos^2 x - 1$:
\[
2\cos x = 2\cos^2 x - 1
\]
\[
2\cos^2 x - 2\cos x - 1 = 0
\]

Rešavamo po $\cos x$:
\[
\cos x = \frac{2 \pm \sqrt{4 + 8}}{4} = \frac{2 \pm \sqrt{12}}{4} = \frac{2 \pm 2\sqrt{3}}{4} = \frac{1 \pm \sqrt{3}}{2}
\]

Pošto $|\cos x| \leq 1$:
\begin{itemize}
\item $\cos x = \frac{1 + \sqrt{3}}{2} \approx \frac{1 + 1.732}{2} \approx 1.366 > 1$ - nije validno
\item $\cos x = \frac{1 - \sqrt{3}}{2} \approx \frac{1 - 1.732}{2} \approx -0.366$ - validno
\end{itemize}

Dakle $\cos x = \frac{1 - \sqrt{3}}{2}$.

Izračunajmo $\cos 2x$:
\[
\cos 2x = 2\cos x = 2 \cdot \frac{1 - \sqrt{3}}{2} = 1 - \sqrt{3}
\]

Izračunajmo $\cos 4x = 2\cos^2 2x - 1$:
\[
\cos^2 2x = (1 - \sqrt{3})^2 = 1 - 2\sqrt{3} + 3 = 4 - 2\sqrt{3}
\]
\[
\cos 4x = 2(4 - 2\sqrt{3}) - 1 = 8 - 4\sqrt{3} - 1 = 7 - 4\sqrt{3}
\]

Iz proporcije $\cos 2x : \cos 4x = 2 : y$:
\[
\frac{\cos 2x}{\cos 4x} = \frac{2}{y}
\]
\[
y = \frac{2\cos 4x}{\cos 2x} = \frac{2(7 - 4\sqrt{3})}{1 - \sqrt{3}}
\]

Racionalizujemo:
\[
y = \frac{2(7 - 4\sqrt{3})(1 + \sqrt{3})}{(1 - \sqrt{3})(1 + \sqrt{3})} = \frac{2(7 - 4\sqrt{3})(1 + \sqrt{3})}{1 - 3} = \frac{2(7 - 4\sqrt{3})(1 + \sqrt{3})}{-2}
\]
\[
= -(7 - 4\sqrt{3})(1 + \sqrt{3}) = -(7 + 7\sqrt{3} - 4\sqrt{3} - 12) = -(-5 + 3\sqrt{3}) = 5 - 3\sqrt{3}
\]

\subsection*{Answer}
$5 - 3\sqrt{3}$ (option \textbf{D}).

\end{document}
