\documentclass[12pt]{article}
\usepackage[margin=1in]{geometry}
\usepackage{amsmath,amssymb}
\begin{document}

\section*{Problem 1}
Za $a\in\mathbb{R}$, $a\neq 3$ izraz
\[
\frac{a^3-27}{(a-3)^2}\cdot \frac{a^2-2a-3}{(a+3)^2-3a}
\]
je jednak:

\subsection*{Solution}
Faktori\u{s}emo:
\[
a^3-27=(a-3)(a^2+3a+9),\qquad a^2-2a-3=(a-3)(a+1),
\]
a
\[
(a+3)^2-3a=a^2+6a+9-3a=a^2+3a+9.
\]
Zato
\[
\frac{a^3-27}{(a-3)^2}=\frac{(a-3)(a^2+3a+9)}{(a-3)^2}=\frac{a^2+3a+9}{a-3},
\]
\[
\frac{a^2-2a-3}{(a+3)^2-3a}=\frac{(a-3)(a+1)}{a^2+3a+9}.
\]
Mno\u{z}enjem i skra\u{c}ivanjem dobijamo
\[
\frac{a^2+3a+9}{a-3}\cdot \frac{(a-3)(a+1)}{a^2+3a+9}=a+1.
\]

\subsection*{Answer}
$a+1$ (option \textbf{C}).

\end{document}


