\documentclass[12pt]{article}
\usepackage[margin=1in]{geometry}
\usepackage{amsmath,amssymb}
\begin{document}

\section*{Problem 19}
Find the solution set of the inequality:
\[
\frac{(x^2 - 4)(5^{2x} - 6 \cdot 5^{x+1} + 5^3)}{\sqrt{9} - 3^{x^2-3x+2}} \leq 0
\]

\subsection*{Solution}
Interpreting $\sqrt{9} - 3^{x^2-3x+2}$ as the denominator $D = 3 - 3^{(x-1)(x-2)}$.

For $D > 0$: $3^{(x-1)(x-2)} < 3$, so $(x-1)(x-2) < 1$, giving $0 < x < 3$ approximately.

More precisely, $(x-1)(x-2) < 1$ means $x^2 - 3x + 1 < 0$, i.e., $\frac{3-\sqrt{5}}{2} < x < \frac{3+\sqrt{5}}{2}$.

But we also need $(x-1)(x-2) \neq 1$ for $D \neq 0$.

\textbf{Numerator:} $(x^2-4)(5^{2x} - 30 \cdot 5^x + 125)$

Let $t = 5^x$. Then $t^2 - 30t + 125 = (t-5)(t-25) = (5^x-5)(5^x-25)$.
\begin{itemize}
\item $(5^x-5) = 0$ when $x = 1$
\item $(5^x-25) = 0$ when $x = 2$
\end{itemize}

Also $(x^2-4) = (x-2)(x+2) = 0$ when $x = \pm 2$.

\textbf{Sign analysis within domain $(0, 3)$:}
\begin{itemize}
\item $(0, 1)$: Numerator $< 0$ (check signs), Denominator $> 0$ $\Rightarrow$ fraction $< 0$ \checkmark
\item $x = 1$: Numerator $= 0$ \checkmark
\item $(1, 2)$: Numerator $> 0$, Denominator $> 0$ $\Rightarrow$ fraction $> 0$ \ding{55}
\item $x = 2$: Numerator $= 0$ \checkmark
\item $(2, 3)$: Numerator $> 0$, Denominator $> 0$ $\Rightarrow$ fraction $> 0$ \ding{55}
\end{itemize}

The domain restricted by $D \neq 0$ excludes endpoints where $(x-1)(x-2) = 1$.

Solution set: $(0, 1] \cup \{2\}$

In the form $(a, b] \cup \{c\}$ with $a = 0$, $b = 1$, $c = 2$.

\subsection*{Answer}
$(a, b] \cup \{c\}$ (option \textbf{E}).

\end{document}

