\documentclass[12pt]{article}
\usepackage[margin=1in]{geometry}
\usepackage{amsmath,amssymb}
\begin{document}

\section*{Problem 1}
For $a \in \mathbb{R}$, $a \neq 3$, simplify the expression:
\[
\frac{a^3 - 27}{(a-3)^2} \cdot \frac{a^2 - 2a - 3}{(a+3)^2 - 3a}
\]

\subsection*{Solution}
First, let's factor each part:

\textbf{Numerator of first fraction:}
\[
a^3 - 27 = (a-3)(a^2 + 3a + 9)
\]

\textbf{Denominator of second fraction:}
\[
(a+3)^2 - 3a = a^2 + 6a + 9 - 3a = a^2 + 3a + 9
\]

\textbf{Numerator of second fraction:}
\[
a^2 - 2a - 3 = (a-3)(a+1)
\]

Substituting these factorizations:
\[
\frac{(a-3)(a^2 + 3a + 9)}{(a-3)^2} \cdot \frac{(a-3)(a+1)}{a^2 + 3a + 9}
\]

Simplifying:
\[
= \frac{a^2 + 3a + 9}{a-3} \cdot \frac{(a-3)(a+1)}{a^2 + 3a + 9} = a + 1
\]

\subsection*{Answer}
$a + 1$ (option \textbf{C}).

\end{document}

