\documentclass[12pt]{article}
\usepackage[margin=1in]{geometry}
\usepackage{amsmath,amssymb}
\begin{document}

\section*{Problem 10}
Find the number of real solutions of the equation:
\[
\sqrt[3]{x-3} + \sqrt[3]{x-1} = \sqrt[3]{2x-4}
\]

\subsection*{Solution}
Let $a = \sqrt[3]{x-3}$ and $b = \sqrt[3]{x-1}$.

Then:
\begin{itemize}
\item $a^3 = x - 3$
\item $b^3 = x - 1$
\item $a^3 + b^3 = (x-3) + (x-1) = 2x - 4$
\end{itemize}

So the equation becomes:
\[
a + b = \sqrt[3]{a^3 + b^3}
\]

Let $s = a + b$. Cubing both sides:
\[
s^3 = a^3 + b^3
\]

Using the identity $a^3 + b^3 = (a+b)(a^2 - ab + b^2) = s(s^2 - 3ab)$:
\[
s^3 = s(s^2 - 3ab) = s^3 - 3abs
\]
\[
3abs = 0
\]

So either $s = 0$ or $ab = 0$.

\textbf{Case 1: $s = 0$} (i.e., $a = -b$)
\[
\sqrt[3]{x-3} = -\sqrt[3]{x-1}
\]
Cubing: $x - 3 = -(x-1) = -x + 1$, so $2x = 4$, $x = 2$.

Check: $\sqrt[3]{-1} + \sqrt[3]{1} = -1 + 1 = 0 = \sqrt[3]{0}$ \checkmark

\textbf{Case 2: $ab = 0$}
\begin{itemize}
\item If $a = 0$: $x - 3 = 0$, so $x = 3$.\\
Check: $0 + \sqrt[3]{2} = \sqrt[3]{2}$ \checkmark
\item If $b = 0$: $x - 1 = 0$, so $x = 1$.\\
Check: $\sqrt[3]{-2} + 0 = \sqrt[3]{-2}$ \checkmark
\end{itemize}

The solutions are $x = 1, 2, 3$, giving \textbf{3 solutions}.

\subsection*{Answer}
$3$ (option \textbf{C}).

\end{document}

