\documentclass[12pt]{article}
\usepackage[margin=1in]{geometry}
\usepackage{amsmath,amssymb}
\begin{document}

\section*{Problem 1}
Vrednost izraza
\[
\left(\frac{(-0{,}4)^3}{(-0{,}8)^3} - \frac{(-0{,}8)^3}{(-0{,}4)^3}\right) : \left(\frac{3}{4} - 3\right)
\]
jednaka je:

(A) $\frac{7}{2}$ \quad (B) $\frac{63}{8}$ \quad (C) $\frac{4}{9}$ \quad (D) $\frac{5}{9}$ \quad (E) $\frac{7}{9}$ \quad (N) Ne znam

\subsection*{Solution}
Let's simplify step by step. First, note that $-0{,}4 = -\frac{2}{5}$ and $-0{,}8 = -\frac{4}{5}$.

So $\frac{-0{,}4}{-0{,}8} = \frac{-2/5}{-4/5} = \frac{1}{2}$.

Therefore:
\[
\frac{(-0{,}4)^3}{(-0{,}8)^3} = \left(\frac{-0{,}4}{-0{,}8}\right)^3 = \left(\frac{1}{2}\right)^3 = \frac{1}{8}
\]

And:
\[
\frac{(-0{,}8)^3}{(-0{,}4)^3} = \left(\frac{-0{,}8}{-0{,}4}\right)^3 = 2^3 = 8
\]

The expression in the first parentheses:
\[
\frac{1}{8} - 8 = \frac{1-64}{8} = -\frac{63}{8}
\]

The expression in the second parentheses:
\[
\frac{3}{4} - 3 = \frac{3-12}{4} = -\frac{9}{4}
\]

Now we divide:
\[
\left(-\frac{63}{8}\right) : \left(-\frac{9}{4}\right) = \frac{63}{8} \cdot \frac{4}{9} = \frac{63 \cdot 4}{8 \cdot 9} = \frac{252}{72} = \frac{7}{2}
\]

\subsection*{Answer}
$\frac{7}{2}$ (option \textbf{A}).

\end{document}
