\documentclass[12pt]{article}
\usepackage[margin=1in]{geometry}
\usepackage{amsmath,amssymb}
\begin{document}

\section*{Problem 11}
Koja od navedenih relacija postoji između rešenja $x_1$ i $x_2$ kvadratne jednačine $x^2 - 6x + 5 + m(x^2 - 5x + 6) = 0$ ($m \in \mathbf{R}$, $m \neq -1$)?

(A) $x_1 + x_2 + 4x_1x_2 = 2$ \quad (B) $x_1 + x_2 + x_1x_2 - 11 = 0$

(C) $x_1 + x_2 - x_1x_2 + 2 = 0$ \quad (D) $x_1 + x_2 - x_1x_2 = 4$

(E) $x_1 + x_2 + 3x_1x_2 = 1$ \quad (N) Ne znam

\subsection*{Solution}
First, let's simplify the equation:
\[
x^2 - 6x + 5 + m(x^2 - 5x + 6) = 0
\]
\[
x^2 - 6x + 5 + mx^2 - 5mx + 6m = 0
\]
\[
(1+m)x^2 - (6+5m)x + (5+6m) = 0
\]

By Vieta's formulas:
\[
x_1 + x_2 = \frac{6+5m}{1+m}
\]
\[
x_1 \cdot x_2 = \frac{5+6m}{1+m}
\]

Let $S = x_1 + x_2$ and $P = x_1 \cdot x_2$.

We need to find a relation between $S$ and $P$ that eliminates $m$.

From $S = \frac{6+5m}{1+m}$:
\[
S(1+m) = 6 + 5m
\]
\[
S + Sm = 6 + 5m
\]
\[
Sm - 5m = 6 - S
\]
\[
m(S - 5) = 6 - S
\]
\[
m = \frac{6-S}{S-5}
\]

From $P = \frac{5+6m}{1+m}$:
\[
P(1+m) = 5 + 6m
\]
\[
P + Pm = 5 + 6m
\]
\[
Pm - 6m = 5 - P
\]
\[
m(P - 6) = 5 - P
\]
\[
m = \frac{5-P}{P-6}
\]

Setting the two expressions for $m$ equal:
\[
\frac{6-S}{S-5} = \frac{5-P}{P-6}
\]

Cross-multiplying:
\[
(6-S)(P-6) = (5-P)(S-5)
\]
\[
6P - 36 - SP + 6S = 5S - 25 - PS + 5P
\]
\[
6P - 36 - SP + 6S = 5S - 25 - PS + 5P
\]
\[
6P - 36 + 6S = 5S - 25 + 5P
\]
\[
P + S = 11
\]

So $x_1 + x_2 + x_1x_2 = 11$, which means $x_1 + x_2 + x_1x_2 - 11 = 0$.

\subsection*{Answer}
$x_1 + x_2 + x_1x_2 - 11 = 0$ (option \textbf{B}).

\end{document}
