\documentclass[12pt]{article}
\usepackage[margin=1in]{geometry}
\usepackage{amsmath,amssymb}
\begin{document}

\section*{Problem 3}
Find the value of $(4 + \sqrt{15})(\sqrt{10} - \sqrt{6})\sqrt{4 - \sqrt{15}}$.

\subsection*{Solution}
Let's denote the expression as:
\[
E = (4 + \sqrt{15})(\sqrt{10} - \sqrt{6})\sqrt{4 - \sqrt{15}}
\]

First, let's work with $\sqrt{4 - \sqrt{15}}$. Notice that:
\[
4 - \sqrt{15} = \frac{16 - 4\sqrt{15}}{4} = \frac{(4)^2 - 4\sqrt{15}}{4}
\]

Let's try to find if $4 - \sqrt{15}$ can be written as a perfect square. 

Let's assume $\sqrt{4 - \sqrt{15}} = \sqrt{a} - \sqrt{b}$ for some positive $a, b$.

Then: $4 - \sqrt{15} = a + b - 2\sqrt{ab}$

Comparing: $a + b = 4$ and $2\sqrt{ab} = \sqrt{15}$, so $4ab = 15$, thus $ab = \frac{15}{4}$.

From $a + b = 4$ and $ab = \frac{15}{4}$, we get the quadratic:
$t^2 - 4t + \frac{15}{4} = 0$

$t = \frac{4 \pm \sqrt{16 - 15}}{2} = \frac{4 \pm 1}{2}$

So $a = \frac{5}{2}$ and $b = \frac{3}{2}$ (or vice versa).

Therefore: $\sqrt{4 - \sqrt{15}} = \sqrt{\frac{5}{2}} - \sqrt{\frac{3}{2}} = \frac{\sqrt{10} - \sqrt{6}}{2}$

Now our expression becomes:
\[
E = (4 + \sqrt{15})(\sqrt{10} - \sqrt{6}) \cdot \frac{\sqrt{10} - \sqrt{6}}{2}
\]

\[
E = \frac{(4 + \sqrt{15})(\sqrt{10} - \sqrt{6})^2}{2}
\]

Let's compute $(\sqrt{10} - \sqrt{6})^2$:
\[
(\sqrt{10} - \sqrt{6})^2 = 10 + 6 - 2\sqrt{60} = 16 - 2\sqrt{60} = 16 - 4\sqrt{15}
\]

So:
\[
E = \frac{(4 + \sqrt{15})(16 - 4\sqrt{15})}{2}
\]

\[
E = \frac{4(4 + \sqrt{15})(4 - \sqrt{15})}{2} = 2(4 + \sqrt{15})(4 - \sqrt{15})
\]

\[
E = 2(16 - 15) = 2 \cdot 1 = 2
\]

\subsection*{Answer}
$2$ (option \textbf{C}).

\end{document}