\documentclass[12pt]{article}
\usepackage[margin=1in]{geometry}
\usepackage{amsmath,amssymb}
\begin{document}

\section*{Problem 8}
Let the function $f_n: \mathbb{R} \to \mathbb{R}$ be defined by $f_1(x) = 2x + 2020$, $f_{n+1}(x) = f_1(f_n(x))$, $n \in \mathbb{N}$. Then $f_{2020}(-2020)$ equals:

\subsection*{Solution}
Let's find the pattern by computing the first few functions:

$f_1(x) = 2x + 2020$

$f_2(x) = f_1(f_1(x)) = f_1(2x + 2020) = 2(2x + 2020) + 2020 = 4x + 4040 + 2020 = 4x + 6060$

$f_3(x) = f_1(f_2(x)) = f_1(4x + 6060) = 2(4x + 6060) + 2020 = 8x + 12120 + 2020 = 8x + 14140$

We can see the pattern:
\begin{align}
f_1(x) &= 2^1 x + 2020 \cdot 1\\
f_2(x) &= 2^2 x + 2020 \cdot 3\\
f_3(x) &= 2^3 x + 2020 \cdot 7
\end{align}

Let's find the general pattern. If $f_n(x) = 2^n x + 2020 \cdot a_n$, then:
\[
f_{n+1}(x) = f_1(f_n(x)) = f_1(2^n x + 2020 \cdot a_n) = 2(2^n x + 2020 \cdot a_n) + 2020
\]
\[
= 2^{n+1} x + 2020 \cdot 2a_n + 2020 = 2^{n+1} x + 2020(2a_n + 1)
\]

So $a_{n+1} = 2a_n + 1$ with $a_1 = 1$.

This gives us:
\begin{align}
a_1 &= 1\\
a_2 &= 2(1) + 1 = 3\\
a_3 &= 2(3) + 1 = 7\\
a_4 &= 2(7) + 1 = 15
\end{align}

We can see that $a_n = 2^n - 1$.

To verify: if $a_n = 2^n - 1$, then $a_{n+1} = 2(2^n - 1) + 1 = 2^{n+1} - 2 + 1 = 2^{n+1} - 1$ âœ“

Therefore:
\[
f_n(x) = 2^n x + 2020(2^n - 1) = 2^n x + 2020 \cdot 2^n - 2020 = 2^n(x + 2020) - 2020
\]

Now we can compute:
\[
f_{2020}(-2020) = 2^{2020}(-2020 + 2020) - 2020 = 2^{2020} \cdot 0 - 2020 = -2020
\]

\subsection*{Answer}
$-2020$ (option \textbf{D}).

\end{document}