\documentclass[12pt]{article}
\usepackage[margin=1in]{geometry}
\usepackage{amsmath,amssymb}
\begin{document}

\section*{Problem 10}
Find the number of real solutions of equation $2x^2 - 6x + \sqrt{x^2 - 3x + 6} + 2 = 0$.

\subsection*{Solution}
Let's rearrange the equation:
\[
2x^2 - 6x + \sqrt{x^2 - 3x + 6} + 2 = 0
\]

\[
\sqrt{x^2 - 3x + 6} = -2x^2 + 6x - 2
\]

For the square root to be defined, we need $x^2 - 3x + 6 \geq 0$.

Let's check the discriminant: $\Delta = (-3)^2 - 4(1)(6) = 9 - 24 = -15 < 0$.

Since the discriminant is negative and the coefficient of $x^2$ is positive, $x^2 - 3x + 6 > 0$ for all real $x$.

So the square root is defined for all real $x$.

For the equation to have solutions, we need:
\[
-2x^2 + 6x - 2 \geq 0
\]

\[
2x^2 - 6x + 2 \leq 0
\]

\[
x^2 - 3x + 1 \leq 0
\]

The discriminant is $\Delta = 9 - 4 = 5 > 0$, so the roots are:
\[
x = \frac{3 \pm \sqrt{5}}{2}
\]

So we need $\frac{3 - \sqrt{5}}{2} \leq x \leq \frac{3 + \sqrt{5}}{2}$.

Now, squaring both sides of our equation (valid since both sides are non-negative in the allowed interval):
\[
x^2 - 3x + 6 = (-2x^2 + 6x - 2)^2
\]

\[
x^2 - 3x + 6 = 4x^4 - 24x^3 + 52x^2 - 24x + 4
\]

\[
0 = 4x^4 - 24x^3 + 51x^2 - 21x - 2
\]

This is a quartic equation. However, we need to check which solutions satisfy our original constraint.

Let's substitute $u = x^2 - 3x + 6$ and $v = -2x^2 + 6x - 2$. We need $u = v^2$ and $v \geq 0$.

Notice that $v = -2(x^2 - 3x + 1)$ and $u = x^2 - 3x + 6 = (x^2 - 3x + 1) + 5$.

Let $w = x^2 - 3x + 1$. Then $u = w + 5$ and $v = -2w$.

We need: $w + 5 = (-2w)^2 = 4w^2$ and $-2w \geq 0$, so $w \leq 0$.

This gives us: $4w^2 - w - 5 = 0$.

Using the quadratic formula: $w = \frac{1 \pm \sqrt{1 + 80}}{8} = \frac{1 \pm 9}{8}$.

So $w = \frac{10}{8} = \frac{5}{4}$ or $w = -1$.

Since we need $w \leq 0$, we take $w = -1$.

So $x^2 - 3x + 1 = -1$, which gives $x^2 - 3x + 2 = 0$.

This factors as $(x-1)(x-2) = 0$, so $x = 1$ or $x = 2$.

Let's verify both solutions in the original equation:

For $x = 1$: $2(1) - 6(1) + \sqrt{1 - 3 + 6} + 2 = 2 - 6 + \sqrt{4} + 2 = 2 - 6 + 2 + 2 = 0$ ✓

For $x = 2$: $2(4) - 6(2) + \sqrt{4 - 6 + 6} + 2 = 8 - 12 + \sqrt{4} + 2 = 8 - 12 + 2 + 2 = 0$ ✓

Both solutions are valid.

\subsection*{Answer}
$2$ (option \textbf{A}).

\end{document}