\documentclass[12pt]{article}
\usepackage[margin=1in]{geometry}
\usepackage{amsmath,amssymb}
\begin{document}

\section*{Problem 16}
Broj realnih rešenja sistema jednačina $x^2 + 3xy + 2y^2 = 0$, $\cos^2 x + \cos^2 y = 1$, za $x \in [-\pi, 0]$ i $y \in [0, \pi]$, je:

(A) 2 \quad (B) 5 \quad (C) veći od 5 \quad (D) 4 \quad (E) 3

\subsection*{Solution}
Prva jednačina:
\[
x^2 + 3xy + 2y^2 = 0
\]
Faktorizujemo:
\[
(x + y)(x + 2y) = 0
\]
Dakle $x = -y$ ili $x = -2y$.

\textbf{Slučaj 1:} $x = -y$

Pošto $x \in [-\pi, 0]$ i $y \in [0, \pi]$, imamo $x = -y$ gde je $y \in [0, \pi]$, dakle $x \in [-\pi, 0]$ ✓

Druga jednačina: $\cos^2(-y) + \cos^2 y = 1 \Rightarrow 2\cos^2 y = 1 \Rightarrow \cos^2 y = \frac{1}{2}$

$\cos y = \pm\frac{\sqrt{2}}{2}$

Za $y \in [0, \pi]$: $y = \frac{\pi}{4}, \frac{3\pi}{4}$ (za $\cos y = \frac{\sqrt{2}}{2}$ i $\cos y = -\frac{\sqrt{2}}{2}$)

Rešenja: $(x, y) = \left(-\frac{\pi}{4}, \frac{\pi}{4}\right)$ i $\left(-\frac{3\pi}{4}, \frac{3\pi}{4}\right)$

\textbf{Slučaj 2:} $x = -2y$

Za $y \in [0, \pi]$, imamo $x = -2y \in [-2\pi, 0]$.

Ali $x \in [-\pi, 0]$, dakle $-2y \geq -\pi \Rightarrow y \leq \frac{\pi}{2}$.

Dakle $y \in \left[0, \frac{\pi}{2}\right]$ i $x = -2y \in [-\pi, 0]$ ✓

Druga jednačina: $\cos^2(-2y) + \cos^2 y = 1 \Rightarrow \cos^2 2y + \cos^2 y = 1$

Koristimo $\cos 2y = 2\cos^2 y - 1$:
\[
(2\cos^2 y - 1)^2 + \cos^2 y = 1
\]
\[
4\cos^4 y - 4\cos^2 y + 1 + \cos^2 y = 1
\]
\[
4\cos^4 y - 3\cos^2 y = 0
\]
\[
\cos^2 y(4\cos^2 y - 3) = 0
\]

$\cos^2 y = 0 \Rightarrow y = \frac{\pi}{2}$ (u intervalu $\left[0, \frac{\pi}{2}\right]$)

$\cos^2 y = \frac{3}{4} \Rightarrow \cos y = \pm\frac{\sqrt{3}}{2}$

Za $y \in \left[0, \frac{\pi}{2}\right]$: $\cos y = \frac{\sqrt{3}}{2} \Rightarrow y = \frac{\pi}{6}$

Rešenja iz slučaja 2:
\begin{itemize}
\item $y = \frac{\pi}{2}$, $x = -\pi$: $(x, y) = (-\pi, \frac{\pi}{2})$
\item $y = \frac{\pi}{6}$, $x = -\frac{\pi}{3}$: $(x, y) = \left(-\frac{\pi}{3}, \frac{\pi}{6}\right)$
\end{itemize}

Ukupno: 4 rešenja.

\subsection*{Answer}
$4$ (opcija \textbf{(D)}).

\end{document}

