\documentclass[12pt]{article}
\usepackage[margin=1in]{geometry}
\usepackage{amsmath,amssymb}
\begin{document}

\section*{Problem 6}
If
\[
\log_2(\sqrt3+1)+\log_2(\sqrt6-2)=A,
\]
compute
\[
\log_{1/4}(\sqrt3-1)+\log_{1/4}(\sqrt6+2).
\]

\subsection*{Solution}
First,
\[
A=\log_2\bigl((\sqrt3+1)(\sqrt6-2)\bigr).
\]
Let
\[
P_1=(\sqrt3+1)(\sqrt6-2),\qquad P_2=(\sqrt3-1)(\sqrt6+2).
\]
Then
\[
P_1P_2=(\sqrt3+1)(\sqrt3-1)\cdot(\sqrt6-2)(\sqrt6+2)
=(3-1)(6-4)=2\cdot 2=4.
\]
Taking $\log_2$ gives
\[
\log_2 P_1+\log_2 P_2=\log_2 4=2
\;\Rightarrow\;
\log_2 P_2=2-A.
\]
Now use $\log_{1/4} x=\dfrac{\log_2 x}{\log_2(1/4)}=\dfrac{\log_2 x}{-2}=-\frac12\log_2 x$:
\[
\log_{1/4}(\sqrt3-1)+\log_{1/4}(\sqrt6+2)
\;=\;-\frac12\log_2\bigl((\sqrt3-1)(\sqrt6+2)\bigr)
\;=\;-\frac12(2-A)=\frac{A}{2}-1.
\]

\subsection*{Answer}
$\dfrac{A}{2}-1$ (option \textbf{D}).

\end{document}

