\documentclass[12pt]{article}
\usepackage[margin=1in]{geometry}
\usepackage{amsmath,amssymb}
\begin{document}

\section*{Problem 12}
In the binomial expansion of $\left(x - \frac{1}{\sqrt[5]{x}}\right)^{12}$ (where $x \in \mathbf{R} \setminus \{0\}$), find the term that does not contain $x$.

Options: (A) $-132$ \quad (B) $66$ \quad (C) $11$ \quad (D) $-12$ \quad (E) $1$ \quad (N) Ne znam

\subsection*{Solution}
Using the binomial theorem:
\[
\left(x - \frac{1}{\sqrt[5]{x}}\right)^{12} = \left(x - x^{-1/5}\right)^{12} = \sum_{k=0}^{12} \binom{12}{k} x^{12-k} \cdot (-x^{-1/5})^k
\]

The general term is:
\[
T_k = \binom{12}{k} x^{12-k} \cdot (-1)^k \cdot x^{-k/5} = \binom{12}{k} (-1)^k x^{12-k-k/5}
\]

Simplify the exponent:
\[
12 - k - \frac{k}{5} = 12 - \frac{6k}{5}
\]

For the term independent of $x$, set the exponent to 0:
\[
12 - \frac{6k}{5} = 0
\]
\[
\frac{6k}{5} = 12
\]
\[
k = 10
\]

The term with $k = 10$:
\[
T_{10} = \binom{12}{10} (-1)^{10} x^0 = \binom{12}{10} \cdot 1 \cdot 1 = \binom{12}{2} = \frac{12 \cdot 11}{2} = 66
\]

\subsection*{Answer}
$66$ (option \textbf{B}).

\end{document}
