\documentclass[12pt]{article}
\usepackage[margin=1in]{geometry}
\usepackage{amsmath,amssymb}
\begin{document}

\section*{Problem 10}
If $f(x) = 2x + |x|$ and $g(x) = \frac{2}{3}x - \frac{1}{3}|x|$, find $f(g(x))$.

Options: (A) $\frac{2}{3}x$ \quad (B) $|x|$ \quad (C) $-x$ \quad (D) $x$ \quad (E) $3x$ \quad (N) Ne znam

\subsection*{Solution}
First, let's simplify $g(x)$ by considering cases.

\textbf{Case 1:} $x \geq 0$, so $|x| = x$
\[
g(x) = \frac{2}{3}x - \frac{1}{3}x = \frac{1}{3}x \geq 0
\]

\textbf{Case 2:} $x < 0$, so $|x| = -x$
\[
g(x) = \frac{2}{3}x - \frac{1}{3}(-x) = \frac{2}{3}x + \frac{1}{3}x = x < 0
\]

Now find $f(g(x))$:

\textbf{Case 1:} $x \geq 0$: $g(x) = \frac{1}{3}x \geq 0$, so $|g(x)| = \frac{1}{3}x$
\[
f(g(x)) = 2 \cdot \frac{1}{3}x + \frac{1}{3}x = \frac{2}{3}x + \frac{1}{3}x = x
\]

\textbf{Case 2:} $x < 0$: $g(x) = x < 0$, so $|g(x)| = -x$
\[
f(g(x)) = 2x + (-x) = x
\]

In both cases, $f(g(x)) = x$.

\subsection*{Answer}
$x$ (option \textbf{D}).

\end{document}
