\documentclass[12pt]{article}
\usepackage[margin=1in]{geometry}
\usepackage{amsmath,amssymb}
\begin{document}

\section*{Problem 3}
Find the value of the expression $\displaystyle\frac{x^{0.5} + 1}{x + x^{0.5} + 1} : \frac{1}{x^{1.5} - 1}$ for $x \geq 0$, $x \neq 1$.

Options: (A) $x^2 - 1$ \quad (B) $2x - 1$ \quad (C) $2\sqrt{x} - 1$ \quad (D) $x - 1$ \quad (E) $\sqrt{x} - 1$ \quad (N) Ne znam

\subsection*{Solution}
Let $t = x^{0.5} = \sqrt{x}$, so $x = t^2$ and $x^{1.5} = t^3$.

The expression becomes:
\[
\frac{t + 1}{t^2 + t + 1} : \frac{1}{t^3 - 1}
\]

Recall that $t^3 - 1 = (t-1)(t^2 + t + 1)$.

So:
\[
\frac{t + 1}{t^2 + t + 1} \cdot (t^3 - 1) = \frac{t + 1}{t^2 + t + 1} \cdot (t-1)(t^2 + t + 1)
\]

The $(t^2 + t + 1)$ terms cancel:
\[
= (t + 1)(t - 1) = t^2 - 1 = x - 1
\]

\subsection*{Answer}
$x - 1$ (option \textbf{D}).

\end{document}
