\documentclass[12pt]{article}
\usepackage[margin=1in]{geometry}
\usepackage{amsmath,amssymb}
\begin{document}

\section*{Problem 5}
Find the remainder when $P(x) = x^{2022} - 2x^{2021} + x^{2019} - x^2 + 2x + 1$ is divided by $Q(x) = x^2 + 1$.

(A) $-2x + 1$ \quad (B) $1$ \quad (C) $-x - 1$ \quad (D) $x - 1$ \quad (E) $-x + 1$

\subsection*{Solution}
When dividing by $Q(x) = x^2 + 1$, the remainder $R(x) = ax + b$ is a polynomial of degree at most 1.

The roots of $Q(x) = x^2 + 1$ are $x = i$ and $x = -i$.

Since $P(x) = Q(x) \cdot S(x) + R(x)$ for some polynomial $S(x)$, we have:
\[
P(i) = R(i) \quad \text{and} \quad P(-i) = R(-i)
\]

\textbf{Calculate powers of $i$:}
\begin{align*}
i^{2022} &= i^{4 \cdot 505 + 2} = i^2 = -1 \\
i^{2021} &= i^{4 \cdot 505 + 1} = i \\
i^{2019} &= i^{4 \cdot 504 + 3} = i^3 = -i
\end{align*}

\textbf{Calculate $P(i)$:}
\begin{align*}
P(i) &= i^{2022} - 2i^{2021} + i^{2019} - i^2 + 2i + 1 \\
&= -1 - 2i + (-i) - (-1) + 2i + 1 \\
&= -1 - 2i - i + 1 + 2i + 1 \\
&= 1 - i
\end{align*}

\textbf{Calculate $P(-i)$:}
\begin{align*}
(-i)^{2022} &= i^{2022} = -1 \\
(-i)^{2021} &= -i^{2021} = -i \\
(-i)^{2019} &= -i^{2019} = -(-i) = i
\end{align*}
\begin{align*}
P(-i) &= -1 - 2(-i) + i - (-1) + 2(-i) + 1 \\
&= -1 + 2i + i + 1 - 2i + 1 \\
&= 1 + i
\end{align*}

\textbf{Find $R(x) = ax + b$:}
\[
R(i) = ai + b = 1 - i
\]
\[
R(-i) = -ai + b = 1 + i
\]

Adding these equations: $2b = 2 \Rightarrow b = 1$

Subtracting: $2ai = -2i \Rightarrow a = -1$

Therefore: $R(x) = -x + 1$

\subsection*{Answer}
$-x + 1$ (option \textbf{E}).

\end{document}
