\documentclass[12pt]{article}
\usepackage[margin=1in]{geometry}
\usepackage{amsmath,amssymb}
\begin{document}

\section*{Problem 3}
Find the value of $\left(3^{\frac{2 - \log_{3\sqrt{3}} 5 + 2\log_9 4}{4}}\right)^6$.

(A) 1 \quad (B) 8/9 \quad (C) 2 \quad (D) 25/9 \quad (E) 216/5

\subsection*{Solution}
\textbf{Step 1:} Convert the logarithms to base 3.

For $\log_{3\sqrt{3}} 5$:
\[
\log_{3\sqrt{3}} 5 = \frac{\log_3 5}{\log_3 (3\sqrt{3})} = \frac{\log_3 5}{\log_3 3 + \log_3 \sqrt{3}} = \frac{\log_3 5}{1 + \frac{1}{2}} = \frac{\log_3 5}{\frac{3}{2}} = \frac{2}{3}\log_3 5
\]

For $\log_9 4$:
\[
\log_9 4 = \frac{\log_3 4}{\log_3 9} = \frac{\log_3 4}{2} = \frac{1}{2}\log_3 4
\]

\textbf{Step 2:} Substitute into the exponent:
\[
\frac{2 - \frac{2}{3}\log_3 5 + 2 \cdot \frac{1}{2}\log_3 4}{4} = \frac{2 - \frac{2}{3}\log_3 5 + \log_3 4}{4}
\]

\textbf{Step 3:} Rewrite using properties of logarithms:
\[
= \frac{\log_3 9 + \log_3 4 - \log_3 5^{2/3}}{4} = \frac{\log_3 \frac{36}{5^{2/3}}}{4} = \frac{1}{4}\log_3 \frac{36}{\sqrt[3]{25}}
\]

\textbf{Step 4:} Calculate $3^{\frac{1}{4}\log_3 \frac{36}{\sqrt[3]{25}}}$:
\[
3^{\frac{1}{4}\log_3 \frac{36}{\sqrt[3]{25}}} = \left(\frac{36}{\sqrt[3]{25}}\right)^{1/4}
\]

\textbf{Step 5:} Raise to the 6th power:
\[
\left[\left(\frac{36}{\sqrt[3]{25}}\right)^{1/4}\right]^6 = \left(\frac{36}{\sqrt[3]{25}}\right)^{3/2}
\]

\textbf{Step 6:} Calculate:
\[
= \frac{36^{3/2}}{25^{1/2}} = \frac{(\sqrt{36})^3}{\sqrt{25}} = \frac{6^3}{5} = \frac{216}{5}
\]

\subsection*{Answer}
$\frac{216}{5}$ (option \textbf{E}).

\end{document}
